proving in CompileStatement.v
--HG--
branch : adt

platform/cito/CompileStatement.v
@@ -129,12 +129,12 @@ Section Compiler.
       | a :: ls' => Seq2 a (Seq ls')
     end.
 
-  Definition SaveRv var := Strline (Assign (variableSlot var vars) (RvLval (LvReg Rv)) :: nil).
+  Definition SaveRv var := Strline (IL.Assign (variableSlot var vars) (RvLval (LvReg Rv)) :: nil).
 
   Local Notation "v [( e )]" := (exprDenote e (fst v)) (no associativity, at level 60).
   
   Definition loop_inv cond body k : assert := 
-    let s := Loop cond body;: k in
+    let s := While cond body;: k in
     st ~> Ex fs, funcsOk layout (fst st) fs /\ ExX, Ex v, Ex res,
     ![^[locals ("rp" :: vars) (fst v) res st#Sp * is_heap layout (snd v) * mallocHeap 0] * #0] st
     /\ [| res = wordToNat (sel (fst v) S_RESERVED) /\ Safe fs s v |]
@@ -165,7 +165,7 @@ Section Compiler.
   Fixpoint put_args base target n :=
     match n with
       | 0 => nil
-      | S n' => Assign (LvMem (Indir Rv (natToW target))) (RvLval (variableSlot (tempOf base) vars)) :: put_args (1 + base) (4 + target) n'
+      | S n' => IL.Assign (LvMem (Indir Rv (natToW target))) (RvLval (variableSlot (tempOf base) vars)) :: put_args (1 + base) (4 + target) n'
     end.
 
   Definition CheckStack n cmd :=
@@ -186,21 +186,21 @@ Section Compiler.
       | Syntax.Seq a b => Seq2 
           (compile a (Syntax.Seq b k))
           (compile b k)
-      | Conditional cond t f => Seq2
+      | Syntax.If cond t f => Seq2
         (exprCmd cond 0)
         (Structured.If_ imports_global 
           (RvLval (LvReg Rv)) IL.Ne (RvImm $0) 
           (compile t k) 
           (compile f k)) 
-      | Loop cond body => Seq2
+      | While cond body => Seq2
         (exprCmd cond 0)
         (Structured.While_ imports_global 
           (loop_inv cond body k)
           (RvLval (LvReg Rv)) IL.Ne (RvImm $0)
           (Seq2
-            (compile body (Syntax.Seq (Syntax.Loop cond body) k))
+            (compile body (Syntax.Seq (Syntax.While cond body) k))
             (exprCmd cond 0)))
-      | Syntax.Assignment var expr => Seq (
+      | Syntax.Assign var expr => Seq (
           exprCmd expr 0 ::
           SaveRv var :: 
           nil)
@@ -215,7 +215,7 @@ Section Compiler.
             :: IL.Binop (LvMem (Indir Rv $4)) (RvLval (variableSlot S_RESERVED vars)) Minus (RvImm (natToW init_frame))
             :: nil
             ++ put_args 1 8 (length args)
-            ++ Assign Rv (RvLval (variableSlot (tempOf 0) vars))
+            ++ IL.Assign Rv (RvLval (variableSlot (tempOf 0) vars))
             :: IL.Binop Sp Sp Plus (natToW (4 * (1 + List.length vars))) 
             :: nil)
           :: Structured.ICall_ _ _ Rv (afterCall k)
@@ -227,27 +227,1710 @@ Section Compiler.
 
   Require Import SemanticsExprLemmas.
   Require Import SemanticsLemmas.
-  Require Import MyMalloc MyFree.
-  Import WMake.
 
-  Opaque heap.
-
-  Ltac unfold_eval := unfold precond, postcond, inv, expr_runs_to, runs_to_generic, vars, MIN_RESERVED in *.
-
-  Lemma add_remove : forall a v, v %in fst a -> a %%= add_arr (remove_arr a v) v (get_arr a v).
-    intros; hnf; simpl; intuition (unfold WDict.upd);
-      try match goal with
-            | [ |- context[if ?E then _ else _] ] => destruct E; subst
-          end; auto using WMake.equiv_symm, del_add.
+  Lemma star_diff_ptrs : forall specs st other p1 p2, interp specs (![p1 =?>1 * p2 =?> 1 * other] st) -> p1 <> p2.
+    rewrite sepFormula_eq.
+    propxFo.
+    subst.
+    unfold smem_get_word in *.
+    simpl in *.
+    case_eq (smem_get p2 x3).
+    intros.
+    clear H6.
+    case_eq (smem_get p2 x6).
+    clear H9.
+    intros.
+    destruct H2.
+    subst.
+    destruct H5.
+    subst.
+    destruct H4.
+    subst.
+    Require Import Bootstrap.
+    eapply disjoint_get_fwd in H2.
+    eauto.
+    erewrite join_Some by eassumption.
+    discriminate.
+    erewrite join_Some by eassumption.
+    discriminate.
+    intros.
+    rewrite H0 in H9.
+    discriminate.
+    intros.
+    rewrite H in H6.
+    discriminate.
   Qed.
 
-  Hint Immediate add_remove.
+  Hint Resolve star_diff_ptrs.
 
-  Lemma add_remove' : forall a v i, safe_access a v i -> a %%= add_arr (remove_arr a v) v (get_arr a v).
+  Ltac hiding tac :=
+    (let P := fresh "P" in
+      match goal with
+        | [ H : Safe ?fs _ _ |- _ ] => set (P := Safe fs) in *
+        | [ H : ?fs ~:~ _ ~~ _ ~~> _ |- _ ] => set (P := RunsToRelax fs) in *
+      end;
+      hiding tac;
+      subst P) || tac.
+
+  Ltac rearrange_stars HEAD :=
+    match goal with
+      H : interp ?SPECS (![?P] ?ST) |- _ =>
+        let OTHER := fresh in 
+          evar (OTHER : HProp); 
+          assert (interp SPECS (![HEAD * OTHER] ST));
+            unfold OTHER in *; clear OTHER;
+              [ hiding ltac:(step auto_ext) | .. ]
+    end.
+
+  Infix "=~*>" := (ptsto32 nil) (at level 30).
+
+  Import MHeap.MSet.
+
+  Ltac auto_apply :=
+    match goal with
+      H : _ |- _ => eapply H
+    end.
+
+  Ltac open_Some := 
+    match goal with
+      H : Some _ = Some _ |- _ => injection H; clear H; intros
+    end.
+
+  Ltac condition_solver :=  
+    match goal with
+      H : evalCond _ _ _ _ _ = Some ?T |- wneb _ _ = ?T => 
+      unfold evalCond in *; simpl in *; open_Some; rewriter_r; f_equal
+    end.
+
+  Open Scope nat.
+
+  Hint Rewrite sum_S : arith.
+  Hint Resolve S_le_lt.
+  Hint Resolve sel_upd_firstn.
+  Hint Resolve firstn_S_upd.
+  Hint Resolve VariableLemmas.noChange.
+  Hint Resolve Max.le_max_l Max.le_max_r.
+  Hint Extern 12 => rv_solver.
+  Hint Extern 12 => sp_solver.
+  Hint Resolve le_plus_lt lt_max_l lt_max_r.
+  Hint Resolve plus_le.
+  Hint Resolve lt_le_S plus_lt.
+
+  Lemma le_max_l_trans : forall a b c, (a <= b -> a <= max b c)%nat.
+    intros; eapply le_trans.
+    2: eapply Max.le_max_l.
+    eauto.
+  Qed.
+  Hint Resolve le_max_l_trans.
+
+  Lemma le_max_r_trans : forall a b c, (a <= c -> a <= max b c)%nat.
+    intros; eapply le_trans.
+    2: eapply Max.le_max_r.
+    eauto.
+  Qed.
+  Hint Resolve le_max_r_trans.
+
+  Ltac max_le_solver :=
+    repeat 
+      match goal with
+        | |- ?A <= ?A => eapply le_n
+        | |- max ?A ?B <= _ => eapply Max.max_lub
+        | |- ?S <= max ?A _ =>
+          match A with
+            context [ S ] => eapply le_max_l_trans
+          end
+        | |- ?S <= max _ ?B =>
+          match B with
+            context [ S ] => eapply le_max_r_trans
+          end
+      end.
+  Hint Extern 0 (_ <= _) => progress max_le_solver.
+
+  Ltac incl_app_solver :=
+    repeat 
+      match goal with
+        | |- List.incl ?A ?A => eapply List.incl_refl
+        | |- List.incl (?A ++ ?B) _ => eapply incl_app
+        | |- List.incl (?A :: ?B) _ => eapply List.incl_cons
+        | |- List.incl ?S (?A ++ _) =>
+          match A with
+            context [ S ] => eapply incl_appl
+          end
+        | |- List.incl ?S (_ ++ ?B) =>
+          match B with
+            context [ S ] => eapply incl_appr
+          end
+        | |- List.incl ?S (?A :: _) =>
+          match A with
+            context [ S ] => eapply (@incl_appl _ _ _ (_ :: nil))
+          end
+        | |- List.incl ?S (?A :: ?B) =>
+          match B with
+            context [ S ] => eapply (@incl_appr _ _ (_ :: nil))
+          end
+      end.
+  Hint Extern 0 (List.incl _ _) => progress incl_app_solver.
+
+  Hint Resolve in_eq In_incl.
+  Hint Resolve List.incl_cons incl_cons_l incl_cons_r List.incl_refl incl_nil incl_tl incl_array.
+  Hint Resolve incl_app incl_appl incl_appr.
+  Hint Resolve List.incl_tran.
+  Hint Resolve disjoint_trans_lr.
+  Hint Resolve changedVariables_upd.
+  Hint Resolve unchanged_in_except_disjoint unchanged_in_except_upd unchanged_in_except_shrink.
+  Hint Constructors or.
+  Hint Resolve sel_upd_eq.
+
+  Hint Constructors RunsTo.
+  Hint Constructors runs_loop_partially.
+  Hint Resolve unchanged_exprDenote.
+  Hint Resolve changedVariables_upd_bwd.
+  Hint Resolve unchanged_incl.
+  Hint Resolve two_merge_equiv.
+  Hint Resolve changed_in_upd_same.
+
+  Hint Extern 12 (unchanged_in _ _ _) => use_changed_unchanged.
+  Hint Extern 12 (unchanged_in _ _ _) => use_changed_unchanged'.
+  Hint Extern 12 (changed_in _ _ _) => use_changed_trans2.
+  Hint Extern 12 (changed_in _ _ _) => use_changed_incl.
+  Hint Extern 12 => condition_solver'.
+  Hint Extern 12 (unchanged_in _ _ _) => use_unchanged_in_symm.
+  Hint Extern 12 (changed_in _ _ _) => use_changed_in_symm.
+
+  Hint Resolve runs_loop_partially_finish.
+  Hint Resolve exprDenote_disjoint.
+  Hint Resolve RunsTo_footprint.
+
+  Hint Extern 12 (_ = _) => condition_solver.
+
+  Ltac use_unchanged_exprDenote :=
+    match goal with
+      |- exprDenote ?E _ = exprDenote ?E _ => eapply unchanged_exprDenote; solve [eauto]
+    end.
+  Hint Extern 12 => use_unchanged_exprDenote.
+
+  Lemma incl_tempChunk2 : forall b n m, b + n <= m -> List.incl (tempChunk b n) (tempVars m).
+    intros; eapply incl_tempChunk; eauto.
+  Qed.
+
+  Hint Resolve incl_tempChunk2.
+
+  Ltac auto_apply_in t :=
+    match goal with
+      H : _ |- _ => eapply t in H
+    end.
+
+  Ltac apply_in_all t :=
+    repeat match goal with
+             H : _ |- _ => eapply t in H
+           end.
+
+  Ltac inv_Safe :=
+    match goal with
+      H : Safe _ _ _ |- _ => inversion H
+    end.
+
+  Ltac break_st := unfold st in *; repeat break_pair; simpl in *.
+
+  Ltac use_Safe_immune :=
+    match goal with
+      H : RunsTo _ _ _ _, H2 : context [RunsTo _ _ _ _ -> Safe _ _ _] |- _ => eapply H2 in H; break_st; eapply Safe_immune
+    end.
+
+  Ltac change_RunsTo :=
+    match goal with
+      H : RunsTo _ _ (?VS1, ?ARRS) _, H2 : changed_in ?VS2 ?VS1 _ |- _ => 
+        generalize H; eapply RunsTo_immune with (vs1' := (VS2, ARRS)) in H; intros
+    end.
+
+  Definition equiv (a b : Heap) := fst a %= fst b /\ forall e, e %in fst a -> snd a e = snd b e.
+
+  Infix "%%=" := equiv (at level 70, no associativity).
+
+  Lemma disjoint_cons : forall A a (e : A) b, ~In e a -> disjoint a b -> disjoint a (e :: b).
+    unfold disj; intros; simpl; intuition; eauto.
+  Qed.
+
+  Lemma disjoint_disj : forall A (a : list A) b, disjoint a b -> disj a b.
+    unfold disj, disj; eauto.
+  Qed.
+
+  Lemma changed_trans_l : forall vs1 vs2 vs3 a c, 
+    changedVariables vs1 vs2 a -> 
+    changedVariables vs2 vs3 c ->
+    List.incl a c ->
+    changedVariables vs1 vs3 c.
+    eauto.
+  Qed.
+
+  Lemma del_not_in : forall s e, ~ e %in s %- e.
+    unfold mem, del; intros; intuition.
+  Qed.
+
+  Ltac is_reg t r :=
+    match t with
+      | _ # r => idtac
+      | Regs _ r => idtac
+    end.
+
+  Ltac sp_solver' := 
+    match goal with
+      |- ?A = ?B => is_reg A Sp; is_reg B Sp; pattern_r; rewriter_r
+    end.
+
+  Hint Extern 12 => sp_solver'.
+
+  Ltac use_disjoint_trans :=
+    match goal with
+      H : disjoint ?A ?B |- disjoint ?C _ =>
+        match A with context [ C ] =>
+          eapply (@disjoint_trans_lr _ A B C _ H); [ | eapply List.incl_refl ]
+        end 
+    end.
+
+  Hint Resolve del_not_in.
+  Hint Resolve temp_in_array.
+  Hint Resolve temps_not_in_array.
+  Hint Resolve true_false_contradict.
+
+  Ltac to_tempOf :=
+    replace "!." with (tempOf 1) in * by eauto;
+      replace "." with (tempOf 0) in * by eauto.
+
+  Lemma del_add : forall s e, e %in s -> s %- e %+ e %= s.
+    clear; intros.
+    set (s %- e).
+    eapply equiv_symm.
+    eapply del_to_add.
+    eauto.
+    unfold s0; eauto.
+  Qed.
+
+  Hint Resolve le_n_S.
+
+  Ltac use_disjoint_trans' :=
+    match goal with
+      H : disjoint ?A ?B |- disjoint ?C _ =>
+        match A with context [ C ] =>
+          eapply (@disjoint_trans_lr _ A B C _ H)
+        end 
+    end.
+
+  Hint Resolve Safe_cond_true Safe_cond_false.
+
+  Ltac decide_constructor :=
+    match goal with
+      H : evalCond _ _ _ _ _ = Some ?B |- RunsTo (Syntax.If _ _ _) _ _ =>
+        match B with
+          | true => econstructor 6
+          | false => econstructor 7
+        end
+    end.
+
+  Hint Extern 1 => decide_constructor.
+
+  Hint Resolve runs_loop_partially_body_safe.
+
+  Hint Resolve Safe_immune.
+
+  Ltac tempOf_solver :=
+    match goal with
+      H : List.incl (tempVars _) ?VARS |- In (tempOf ?N) ?VARS =>
+        eapply In_incl; [eapply temp_in_array with (n := S N); omega | eapply incl_tran with (2 := H) ]
+    end.
+
+  Hint Extern 1 => tempOf_solver.
+
+  Opaque tempVars.
+
+  Ltac incl_tran_tempVars :=
+    match goal with
+      H : List.incl (tempVars _) ?VARS |- List.incl (tempVars _) ?VARS => eapply incl_tran with (2 := H)
+    end.
+
+  Hint Extern 1 => incl_tran_tempVars.
+
+  Ltac clear_step := try clear_imports; step auto_ext.
+
+  Ltac in_solver :=
+    match goal with
+      H : Safe _ _ (_, ?ARRS) |- _ %in fst ?ARRS => rewriter; inv_Safe
+    end.
+
+  Hint Extern 1 => in_solver.
+
+  Ltac use_Safe_immune2 :=
+    match goal with
+      | H : Safe _ ?S_H (?VS1, ?ARRS), H2 : changed_in ?VS1 ?VS2 _ |- Safe _ ?S_G (?VS2, ?ARRS) =>
+        match S_H with
+          context [ S_G ] => eapply (@Safe_immune _ S_G VS1 VS2 ARRS); [ | simpl; use_changed_unchanged; use_disjoint_trans']
+        end
+      | H : Safe _ (Syntax.Seq ?A ?B) ?V, H2 : RunsTo _ ?A ?V ?V' |- Safe _ ?B _ => break_st; rewriter; eapply Safe_immune
+      | H : Safe _ (While ?E ?B) _, H2 : runs_loop_partially ?E ?B _ _ |- Safe _ ?B _ => break_st; rewriter; eapply Safe_immune; [ eapply (@runs_loop_partially_body_safe _ _ _ _ _ H2) | ]; [ try use_Safe_immune2 | .. ]
+    end.
+
+  Lemma Safe_seq_first : forall fs a b v, Safe fs (Syntax.Seq a b) v -> Safe fs a v.
+    intros; inv_Safe; eauto.
+  Qed.
+
+  Hint Resolve Safe_seq_first.
+
+  Lemma unchanged_in_refl : forall vs vars, unchanged_in vs vs vars.
+    unfold unchanged_in; eauto.
+  Qed.
+
+  Hint Resolve unchanged_in_refl.
+
+  Lemma Safe_seq_second : forall fs a b v v', Safe fs (Syntax.Seq a b) v -> RunsTo fs a v v' -> Safe fs b v'.
+    intros; inv_Safe; use_Safe_immune; eauto.
+  Qed.
+
+  Hint Resolve Safe_seq_second.
+
+  Ltac change_RunsTo_arrs :=
+    match goal with
+      H : RunsTo _ ?S (?VS, ?ARRS1) _ |- RunsTo _ ?S (?VS, ?ARRS2) _ => replace ARRS2 with ARRS1
+    end.
+
+  Hint Extern 1 => change_RunsTo_arrs.
+
+  Ltac extend_runs_loop_partially :=
+    match goal with
+      H : runs_loop_partially _ ?E ?B ?V (?VS, _), H2 : RunsTo _ ?B (?VS, _) ?V'' |- runs_loop_partially _ ?E ?B ?V _ =>
+        eapply (@LoopPartialStep _ _ _ _ _ V'' H)
+    end.
+
+  Ltac use_changed_in_eval :=
+    match goal with
+      H : VariableLemmas.equiv ?V (merge _ _ _) |- changed_in ?V _ _ =>
+        apply_in_all RunsTo_footprint; eapply changed_in_eval; [eassumption | ..]
+    end.
+
+  Ltac pre_descend := first [change_RunsTo | auto_apply_in runs_loop_partially_finish; [change_RunsTo | ..] ]; open_hyp; break_st.
+
+  Ltac arrays_eq_solver :=
+    match goal with
+      |- ?A = _ =>
+      match type of A with
+        Heap => simpl in *; congruence
+      end
+    end.
+
+  Ltac choose_changed_unchanged :=
+    match goal with
+      H : disjoint ?A ?B |- unchanged_in _ _ ?C =>
+        match A with
+          context [ C ] => eapply (@changed_unchanged _ _ B _)
+        end
+    end.
+
+  Ltac iter_changed_discharger := first [eassumption | eapply changedVariables_incl; [eassumption | ..] | eapply changedVariables_upd_fwd | eapply changedVariables_incl; [eapply changedVariables_upd_fwd | ..] ].
+
+  Ltac iter_changed := repeat first [iter_changed_discharger | eapply changed_trans_l].
+
+  Ltac format_solver :=
+    match goal with
+      |- _ = exprDenote _ _ ^+ $4 ^* exprDenote _ _ =>
+      rewriter; erewrite changed_in_inv by eauto; rewrite sel_upd_eq by eauto; rewriter; repeat (f_equal; try (eapply unchanged_exprDenote; choose_changed_unchanged; iter_changed))
+    end.
+
+  Opaque List.incl.
+
+  Lemma changed_in_upd_eq : forall vs1 vs2 vars s val1 val2,
+    changed_in vs1 vs2 vars ->
+    val2 = val1 ->
+    changed_in (upd vs1 s val1) (upd vs2 s val2) vars.
+    intros; rewriter; eauto.
+  Qed.
+
+  Hint Resolve changed_in_upd_eq.
+
+  Ltac use_changed_in_upd_same :=
+    match goal with
+      |- changed_in (upd _ ?S _) (upd _ ?S _) _ => eapply changed_in_upd_same; iter_changed
+    end.
+
+  Ltac auto_unfold :=
+    repeat match goal with
+             t := _ |- _ => unfold t in *; clear t
+           end.
+
+  Hint Resolve del_add.
+
+  Hint Resolve equiv_symm.
+
+  Ltac max_2_plus :=
+    match goal with
+      |- (max _ _ >= 2 + _)%nat => simpl
+    end.
+
+  Hint Extern 1 => max_2_plus.
+
+  Ltac tempOf_neq :=
+    match goal with
+      |- ~ (tempOf _ = tempOf _) => discriminate
+    end.
+
+  Hint Extern 1 => tempOf_neq.
+
+  Ltac not_in_solver :=
+    match goal with 
+      H : ?ARRS = _ |- ~ _ %in fst ?ARRS => rewriter
+    end.
+
+  Ltac no_question_mark :=
+    match goal with
+      |- ?T => match T with T => idtac end
+    end.
+
+  Ltac upd_chain_solver :=
+    match goal with
+      H1 : changed_in _ _ _, H2 : changed_in (upd _ _ _) _ _, H3 : changed_in (upd _ _ _) _ _ |- changed_in _ _ _ => no_question_mark; simpl; iter_changed
+    end.
+
+  Ltac rv_length_solver :=
+    match goal with
+      H : Regs ?ST Rv = natToW (length _) |- Regs ?ST Rv = natToW (length _) => rewriter
+    end.
+
+  Hint Extern 1 => rv_length_solver.
+
+  Ltac arrays_eq_solver2 :=
+    match goal with
+      H : ?A = _ |- ?A = _ =>
+        match type of A with
+          Heap => rewriter
+        end
+    end.
+
+  Lemma RunsToRelax_loop_false : forall fs e b k v1 v2, 
+    fs ~:~ v1 ~~ k ~~> v2 -> 
+    wneb (v1[(e)]) $0 = false -> 
+    fs ~:~ v1 ~~ While e b;: k ~~> v2.
+    unfold RunsToRelax; intros; openhyp; descend; eauto.
+  Qed.
+  Hint Resolve RunsToRelax_loop_false.
+
+  Hint Constructors Safe.
+  Lemma Safe_cond_true_k : forall fs e t f k v, 
+    Safe fs (Syntax.If e t f;: k) v ->
+    wneb (v[(e)]) $0 = true ->
+    Safe fs (t;: k) v.
+    inversion 1; intros; econstructor.
+(*here*)
+eapply Safe_seq_first.
+ apply Safety.Seq.
+  eapply Safe_cond_true.
+   exact H2.
+   exact H5.
+   intro.
+   intro.
+   apply Assign.
+
+eapply Safe_seq_first.
+
+ apply Safety.Seq.
+
+  eapply Safe_cond_true.
+
+   exact H2.
+
+   exact H5.
+
+   intro.
+
+   exact H5.
+
+   intro.
+
+   intro.
+
+   apply Assign.
+
+
+  eapply Safe_cond_true.
+
+   exact H2.
+
+   exact H5.
+
+    eauto.
+  Qed.
+  Hint Resolve Safe_cond_true_k.
+  Lemma Safe_cond_false_k : forall fs e t f k v, 
+    Safe fs (Syntax.If e t f;: k) v ->
+    wneb (v[(e)]) $0 = false ->
+    Safe fs (f;: k) v.
+    inversion 1; intros; econstructor; eauto.
+    Grab Existential Variables.
+    eauto.
+    eauto.
+  Qed.
+  Hint Resolve Safe_cond_false_k.
+
+  Ltac use_disjoint_trans'' := 
+    match goal with
+      | H : disjoint ?A ?B |- disjoint ?C _ =>
+        match A with context [ C ] =>
+          eapply (@disjoint_trans_lr _ A B C _ H)
+        end 
+      | H : disjoint ?A ?B |- disjoint (?C1 ++ ?C2) _ =>
+        match A with context [ C1 ] =>
+          match A with context [ C2 ] =>
+            eapply (@disjoint_trans_lr _ A B (C1 ++ C2) _ H)
+          end
+        end 
+    end.
+  Hint Extern 1 => use_disjoint_trans''.
+
+  Ltac change_rp :=
+    match goal with
+      H : ?SPECS (sel ?VS1 "rp") = Some _ |- ?SPECS (sel ?VS2 "rp") = Some _ =>
+        replace (sel VS2 "rp") with (sel VS1 "rp") by (symmetry; eapply changed_in_inv; [ eauto | ]; eapply in_tran_not; [ | eauto ]; eapply incl_tran; [ | eassumption ]; eauto)
+    end.
+  Local Notation "'tmps' s" := (tempVars (depth s)) (at level 60).
+  Local Notation "'etmps' s" := (tempVars (edepth s)) (at level 60).
+  Ltac change_RunsTo_for_goal :=
+    match goal with
+      H : RunsTo _ ?S ?VS1 _ |- context [ RunsTo _ ?S ?VS1' _ ] => generalize H; eapply RunsTo_immune with (vs1' := VS1') in H; intros
+    end.
+
+  Local Notation agree_in := unchanged_in.
+  Local Notation agree_except := changed_in.
+  Definition st_agree_except (v1 v2 : st) vars := agree_except (fst v1) (fst v2) vars /\ snd v1 = snd v2.
+  Local Notation "b [ vars => c ]" := (merge c b vars) (no associativity, at level 60).
+  Infix "==" := VariableLemmas.equiv.
+  Local Notation "v1 =~= v2 [^ except ]" := (st_agree_except v1 v2 except) (no associativity, at level 60).
+
+  Lemma st_agree_except_symm : forall v1 v2 ex, v1 =~= v2 [^ex] -> v2 =~= v1 [^ex].
+    unfold st_agree_except; intuition.
+  Qed.
+  Lemma RunsToRelax_immune : forall fs s v1 v2 v1' v2', 
+    fs ~:~ v1 ~~ s ~~> v2 ->
+    v1' =~= v1 [^ tmps s] -> 
+    v2' =~= v2 [^ tmps s] ->
+    disjoint (footprint s) (tmps s) ->
+    fs ~:~ v1' ~~ s ~~> v2'.
+    intros; eapply st_agree_except_symm in H0; eapply st_agree_except_symm in H1; unfold st_agree_except, RunsToRelax in *; openhyp; change_RunsTo_for_goal; eauto; openhyp; descend.
+    eauto.
+    use_changed_in_eval; eauto; eapply changedVariables_symm in H0; eauto.
+    congruence.
+  Qed.
+  Ltac change_RunsTo_to t :=
+    match goal with
+      H : RunsTo _ ?S ?VS1 _ |- _ => generalize H; eapply RunsTo_immune with (vs1' := t) in H; intros
+    end.
+  Local Notation "fs -:- v1 -- s --> v2" := (RunsTo fs s v1 v2) (no associativity, at level 60).
+  Lemma inversion_RunsTo_seq : forall fs a b v1 v2, fs -:- v1 -- a;: b --> v2 -> exists v, fs -:- v1 -- a --> v /\ fs -:- v -- b --> v2.
     inversion 1; eauto.
   Qed.
+  Hint Resolve Max.max_lub.
+  Lemma st_agree_except_refl : forall v ex, v =~= v [^ex].
+    unfold st_agree_except; eauto.
+  Qed.
+  Hint Resolve st_agree_except_refl.
+  Lemma RunsToRelax_cond_true' : forall fs e t f k v1 v2,
+    fs ~:~ v1 ~~ t;: k ~~> v2 ->
+    wneb (v1[(e)]) $0 = true ->
+    fs ~:~ v1 ~~ Syntax.If e t f;: k ~~> v2.
+    unfold RunsToRelax; intros; openhyp; auto_apply_in inversion_RunsTo_seq; openhyp; descend; simpl in *; eauto 6.
+  Qed.
+  Hint Resolve RunsToRelax_cond_true'.
+  Lemma RunsToRelax_cond_true : forall fs e t f k v1 v1' v2,
+    let s := Syntax.If e t f;: k in
+      fs ~:~ v1 ~~ t;: k ~~> v2 ->
+      v1' =~= v1 [^etmps e] ->
+      wneb (v1'[(e)]) $0 = true ->
+      disjoint (footprint s) (tmps s) ->
+      fs ~:~ v1' ~~ s ~~> v2.
+    admit.
+(*    intros; eapply RunsToRelax_immune; unfold s, st_agree_except in *; openhyp; descend; simpl in *; eauto.*)
+  Qed.
+  Lemma RunsToRelax_cond_false' : forall fs e t f k v1 v2,
+    fs ~:~ v1 ~~ f;: k ~~> v2 ->
+    wneb (v1[(e)]) $0 = false ->
+    fs ~:~ v1 ~~ Syntax.If e t f;: k ~~> v2.
+    unfold RunsToRelax; intros; openhyp; auto_apply_in inversion_RunsTo_seq; openhyp; descend; simpl in *; eauto 6.
+  Qed.
+  Hint Resolve RunsToRelax_cond_false'.
+  Lemma RunsToRelax_cond_false : forall fs e t f k v1 v1' v2,
+    let s := Syntax.If e t f;: k in
+      fs ~:~ v1 ~~ f;: k ~~> v2 ->
+      v1' =~= v1 [^etmps e] ->
+      wneb (v1'[(e)]) $0 = false ->
+      disjoint (footprint s) (tmps s) ->
+      fs ~:~ v1' ~~ s ~~> v2.
+    admit.
+(*    intros; eapply RunsToRelax_immune; unfold s, st_agree_except in *; openhyp; descend; simpl in *; eauto.*)
+  Qed.
+  Hint Unfold st_agree_except.
+  Hint Resolve RunsToRelax_cond_true RunsToRelax_cond_false.
 
-  Hint Immediate add_remove'.
+  Local Notation "v [ e ]" := (exprDenote e v) (no associativity, at level 60).
+  Lemma Safe_assign : forall fs var e k vs arrs,
+    Safe fs (var <- e;: k) (vs, arrs)
+    -> Safe fs k (upd vs var (vs[e]), arrs).
+    inversion 1; eauto.
+  Qed.
+  Lemma in_not_in_ne : forall A ls (a b : A), In a ls -> ~ In b ls -> a <> b.
+    intuition.
+  Qed.
+
+  Fixpoint denote_sem s (v : st) := 
+    match s with
+      | var <- e => (upd (fst v) var (fst v[e]), snd v)
+      | _ => v
+    end.
+
+  Lemma RunsToRelax_assign : forall fs var e k v1 v2 v3,
+    fs ~:~ v2 ~~ k ~~> v3 ->
+    denote_sem (var <- e) v1 =~= v2 [^etmps e] ->
+    disjoint (footprint k) (etmps e) ->
+    fs ~:~ v1 ~~ var <- e;: k ~~> v3.
+    intros; eapply st_agree_except_symm in H0; unfold denote_sem, RunsToRelax, st_agree_except in *; openhyp; change_RunsTo_to (denote_sem (var <- e) v1); eauto; openhyp; destruct v1; simpl in *; descend.
+    eauto.
+    eapply changedVariables_symm in H0; use_changed_in_eval; eauto.
+    congruence.
+  Qed.
+
+  Lemma Safe_assoc_left : forall fs a b c v, Safe fs (a;: b;: c) v -> Safe fs (a;: (b;: c)) v.
+    clear; intros; inv_Safe; subst; inversion H; subst; econstructor; [ | intros; econstructor ].
+    eauto.
+    eauto.
+    info_eauto.
+    Grab Existential Variables.
+    eauto.
+    eauto.
+  Qed.
+  Ltac true_not_false :=
+    match goal with
+      H1 : ?A = true, H2 : ?A = false |- _ => eapply Bool.eq_true_false_abs in H1; intuition
+    end.
+  Hint Extern 1 => true_not_false.
+  Lemma Safe_loop_true : forall fs e b v,
+    Safe fs (While e b) v ->
+    wneb (v[(e)]) $0 = true ->
+    Safe fs (b;: While e b) v.
+    intros.
+    inv_Safe.
+    unfold statement0 in *.
+    rewrite <- H2 in *.
+    eauto.
+    eauto.
+  Qed.
+  Hint Resolve Safe_loop_true.
+  Lemma RunsTo_loop_true : forall fs e b v1 v2,
+    fs -:- v1 -- b;: While e b --> v2 ->
+    wneb (v1[(e)]) $0 = true ->
+    fs -:- v1 -- While e b --> v2.
+    clear; intros; eapply inversion_RunsTo_seq in H; openhyp; eauto.
+  Qed.
+  Hint Resolve RunsTo_loop_true.
+  Lemma Safe_loop_true_k : forall fs e b k v, 
+    Safe fs (While e b;: k) v ->
+    wneb (v[(e)]) $0 = true ->
+    Safe fs (b;: (While e b;: k)) v.
+    intros.
+    inv_Safe.
+    subst.
+    inversion H3; try (unfold vals in *; congruence).
+    subst b.
+    subst v.
+    econstructor.
+    eauto.
+    intros.
+    econstructor; eauto.
+  Qed.
+  Hint Resolve Safe_loop_true_k.
+  Local Notation agree_except_trans := changedVariables_trans.
+  Definition tmps_diff big small := tempChunk (depth small) (depth big - depth small).
+  Lemma agree_except_app_comm : forall vs1 vs2 a b,
+    agree_except vs1 vs2 (a ++ b) ->
+    agree_except vs1 vs2 (b ++ a).
+    intros; eauto.
+  Qed.
+  Lemma merge_comm : forall v vars1 v1 vars2 v2,
+    disjoint vars1 vars2 ->
+    v [vars1 => v1] [vars2 => v2] == v [vars2 => v2] [vars1 => v1].
+    intros.
+    unfold VariableLemmas.equiv, changedVariables.
+    intros.
+    contradict H0.
+    destruct (In_dec string_dec x vars1).
+    destruct (In_dec string_dec x vars2).
+    unfold disj in *.
+    contradict H.
+    eauto.
+    rewrite sel_merge by eauto.
+    rewrite sel_merge_outside by eauto.
+    rewrite sel_merge by eauto.
+    eauto.
+    destruct (In_dec string_dec x vars2).
+    rewrite sel_merge_outside by eauto.
+    rewrite sel_merge by eauto.
+    rewrite sel_merge by eauto.
+    eauto.
+    rewrite sel_merge_outside by eauto.
+    rewrite sel_merge_outside by eauto.
+    rewrite sel_merge_outside by eauto.
+    rewrite sel_merge_outside by eauto.
+    eauto.
+  Qed.
+  Lemma equiv_merge_equiv : forall v1 v2 vars v,
+    v1 == v2 ->
+    v1 [vars => v] == v2 [vars => v].
+    intros; eapply two_merge_equiv; eauto.
+  Qed.
+  Lemma RunsToRelax_seq_fwd : forall fs a b v1 v2,
+    fs ~:~ v1 ~~ a;: b ~~> v2 ->
+    disjoint (footprint (a;: b)) (tmps (a;: b)) ->
+    exists v, fs ~:~ v1 ~~ a ~~> v /\ fs ~:~ v ~~ b ~~> v2.
+    clear.
+    unfold RunsToRelax; intros.
+    openhyp.
+    eapply inversion_RunsTo_seq in H.
+    openhyp.
+    simpl in *.
+    destruct (le_lt_dec (depth a) (depth b)).
+    exists (fst x0 [tmps a => fst v2], snd x0).
+    split.
+    descend; eauto.
+    eapply changed_merge_fwd.
+    change_RunsTo_for_goal.
+    openhyp.
+    simpl in *.
+    descend; eauto.
+    use_changed_in_eval.
+    eapply changed_trans_l.
+    eapply changed_merge_bwd.
+    eauto.
+    eauto.
+    eauto.
+    congruence.
+    simpl.
+    eapply changed_unchanged.
+    eapply changed_merge_fwd.
+    eauto.
+    eauto.
+    set (diff := tmps_diff a b).
+    exists (fst x0 [diff => fst v2], snd x0).
+    split.
+    descend; eauto.
+    eapply agree_except_trans.
+    2 : eapply changed_merge_fwd.
+    eauto.
+    eauto.
+    unfold diff, tmps_diff.
+    eapply incl_tempChunk2.
+    omega.
+    change_RunsTo_for_goal.
+    openhyp.
+    simpl in *.
+    descend; eauto.
+    eapply changed_trans_l.
+    Focus 2.
+    eapply changed_merge.
+    eapply agree_except_app_comm.
+    rewrite Max.max_l in * by eauto.
+    erewrite <- split_tmps.
+    eauto.
+    eauto.
+    2 : eapply List.incl_refl.
+    eapply changedVariables_incl.
+    2 : eauto.
+    eapply VariableLemmas.equiv_trans.
+    eauto.
+    apply_in_all RunsTo_footprint.
+    eapply VariableLemmas.equiv_trans.
+    eapply VariableLemmas.equiv_symm.
+    eapply merge_comm.
+    unfold diff, tmps_diff.
+    eauto.
+    unfold diff, tmps_diff.
+    eapply equiv_merge_equiv.
+    eapply changed_merge.
+    eauto.
+    congruence.
+    simpl.
+    unfold diff, tmps_diff.
+    eapply changed_unchanged.
+    eapply changed_merge_fwd.
+    eauto.
+    eauto.
+  Qed.
+  Lemma RunsToRelax_seq_bwd : forall fs a b v1 v2 v3,
+    fs ~:~ v1 ~~ a ~~> v2 ->
+    fs ~:~ v2 ~~ b ~~> v3 ->
+    disjoint (footprint (a;: b)) (tmps (a;: b)) ->
+    fs ~:~ v1 ~~ a;: b ~~> v3.
+    unfold RunsToRelax; intros; openhyp; generalize dependent H; simpl in *; change_RunsTo_to x0; eauto; openhyp; descend; eauto; try use_changed_in_eval; eauto.
+    congruence.
+  Qed.
+  Hint Resolve RunsToRelax_seq_bwd.
+  Lemma RunsToRelax_assoc_left : forall fs a b c v1 v2,
+    fs ~:~ v1 ~~ a;: (b;: c) ~~> v2 ->
+    disjoint (footprint (a;: (b;: c))) (tmps (a;: (b;: c))) ->
+    fs ~:~ v1 ~~ a;: b;: c ~~> v2.
+    clear; simpl; intros; eapply RunsToRelax_seq_fwd in H; eauto; openhyp; eapply RunsToRelax_seq_fwd in H1; eauto; openhyp; repeat eapply RunsToRelax_seq_bwd; repeat (simpl; eauto).
+  Qed.
+  Lemma RunsToRelax_loop_true : forall fs e b v1 v2, 
+    fs ~:~ v1 ~~ b;: While e b ~~> v2 -> 
+    wneb (v1[(e)]) $0 = true -> 
+    fs ~:~ v1 ~~ While e b ~~> v2.
+    unfold RunsToRelax; intros; openhyp; simpl in *; descend; eauto.
+  Qed.
+  Hint Resolve RunsToRelax_loop_true.
+  Lemma RunsToRelax_loop_true_k : forall fs e b k v1 v2, 
+    let s := While e b;: k in
+      fs ~:~ v1 ~~ b;: s ~~> v2 -> 
+      wneb (v1[(e)]) $0 = true -> 
+      disjoint (footprint s) (tmps s) ->
+      fs ~:~ v1 ~~ s ~~> v2.
+    simpl; intros; eapply RunsToRelax_assoc_left in H; simpl; eauto; eapply RunsToRelax_seq_fwd in H; simpl; eauto; openhyp; eauto.
+  Qed.
+  Hint Resolve RunsToRelax_loop_true_k.
+
+  Hint Resolve Safe_assoc_left.
+
+  Lemma RunsToRelax_skip : forall fs s v1 v2,
+    fs ~:~ v1 ~~ s ~~> v2 ->
+    fs ~:~ v1 ~~ skip;: s ~~> v2.
+    unfold RunsToRelax; intros; openhyp; descend; eauto.
+  Qed.
+  Hint Resolve RunsToRelax_skip.
+
+  Lemma mult_S_distr : forall a b, a * S b = a + a * b.
+    intros; ring.
+  Qed.
+
+  Opaque star. (* necessary to use eapply_cancel *)
+
+  Ltac eapply_cancel h specs st := let HP := fresh in let Hnew := fresh in
+    evar (HP : HProp); assert (interp specs (![HP] st)) as Hnew;
+      [ | eapply h in Hnew; [ | clear Hnew .. ] ]; unfold HP in *; clear HP; 
+        [ solve [try clear_imports; hiding ltac:(step auto_ext) ] | .. ].
+
+  Ltac transit := 
+    match goal with
+      | H_interp : interp _ _, H : _ |- _ => eapply H in H_interp; clear H
+      | H_interp : interp ?SPECS (![_] ?ST), H : context [interp _ (![_] ?ST) -> _] |- _ => eapply_cancel H SPECS ST; clear H H_interp
+    end.
+
+  Ltac try_post :=
+    try match goal with
+      H_interp : interp _ ?P |- _ =>
+        match P with
+          | context [ Exists ] => post
+        end
+    end.
+
+  Lemma pack_pair' : forall A B (x : A * B), (let (x, _) := x in x, let (_, y) := x in y) = x.
+    destruct x; simpl; intuition.
+  Qed.
+
+  Lemma fold_second : forall A B (p : A * B), (let (_, y) := p in y) = snd p.
+    destruct p; simpl; intuition.
+  Qed.
+
+  Lemma fold_first : forall A B (p : A * B), (let (x, _) := p in x) = fst p.
+    destruct p; simpl; intuition.
+  Qed.
+
+  Ltac post_step := repeat first [ rewrite pack_pair' in * | rewrite fold_second in * | rewrite fold_first in *].
+
+  Ltac not_mem_rv INST := 
+    match INST with
+      | context [LvMem ?LOC] =>
+        match LOC with
+          | context [Rv] => fail 2
+          | _ => idtac
+        end
+      | _ => idtac
+    end.
+
+  Ltac pre_eval_auto := 
+    repeat 
+      match goal with
+        | H_eval : evalInstrs _ ?ST ?INST = _, H_interp : interp _ (![?P] (_, ?ST)) |- _ =>
+          match INST with
+            context [ Rv ] => 
+            match goal with
+              H_rv : Regs ST Rv = _ |- _ => not_mem_rv INST; post_step; generalize dependent H_rv
+            end
+          end
+        | H_eval : evalInstrs _ ?ST ?INST = _, H_interp : interp _ (![?P] (_, ?ST)) |- _ =>
+          match P with
+            context [ heap ?HEAP ] => 
+            match goal with
+              H_heap : HEAP = _ |- _ => post_step; generalize dependent H_heap
+            end
+          end
+      end.
+
+  Ltac evaluate_hints hints :=
+    match goal with
+      H : evalInstrs _ ?ST _ = _ |- _ => generalize dependent H; evaluate hints; intro; evaluate auto_ext
+    end.
+
+  Ltac my_evaluate hints :=
+    match goal with
+      | H: interp _ (![_](_, ?ST)), H_eval: evalInstrs _ ?ST ?INST = _ |- _  =>
+        match INST with
+          | context [LvMem (Reg Rv) ] => evaluate_hints hints
+          | _ => pre_eval_auto; evaluate hints
+        end
+    end.
+
+  Ltac simpl_sp :=
+    repeat match goal with
+             H : (_, _) # Sp = _ |- _ => simpl in H
+           end.
+
+  Ltac fold_length := 
+    change (fix length (l : list string) : nat :=
+      match l with
+        | nil => 0
+        | _ :: l' => S (length l')
+      end) with (@length string) in *.
+
+  Lemma fold_4S : forall n, (S (S (S (S (4 * n))))) = (4 + (4 * n)).
+    eauto.
+  Qed.
+
+  Lemma Safe_ReadAt_safe_access : forall fs var arr idx v, 
+    Safe fs (Syntax.ReadAt var arr idx) v ->
+    safe_access (snd v) (exprDenote arr (fst v)) (exprDenote idx (fst v)).
+    intros; inv_Safe_clear; eauto.
+  Qed.
+
+  Lemma Safe_WriteAt_safe_access : forall fs arr idx val v, 
+    Safe fs (Syntax.WriteAt arr idx val) v ->
+    safe_access (snd v) (exprDenote arr (fst v)) (exprDenote idx (fst v)).
+    intros; inv_Safe_clear; eauto.
+  Qed.
+
+  Lemma Safe_ReadAt_k_safe_access : forall fs var arr idx v k, 
+    Safe fs (Syntax.ReadAt var arr idx;: k) v ->
+    safe_access (snd v) (exprDenote arr (fst v)) (exprDenote idx (fst v)).
+    intros; eapply Safe_seq_first in H; inv_Safe_clear; eauto.
+  Qed.
+
+  Lemma Safe_WriteAt_k_safe_access : forall fs arr idx val v k, 
+    Safe fs (Syntax.WriteAt arr idx val;: k) v ->
+    safe_access (snd v) (exprDenote arr (fst v)) (exprDenote idx (fst v)).
+    intros; eapply Safe_seq_first in H; inv_Safe_clear; eauto.
+  Qed.
+
+  Ltac not_exist t :=
+    match goal with
+      | H : t |- _ => fail 1
+      | |- _ => idtac
+    end.
+
+  Ltac assert_new t := not_exist t; assert t.
+
+  Ltac assert_new_as t name := not_exist t; assert t as name.
+
+  Definition heap_tag arrs (_ _ : W) := heap arrs.
+
+  Ltac set_all t := let name := fresh "t" in set (name := t) in *.
+
+  Ltac clear_bad H_interp s :=
+    repeat 
+      match goal with
+        | H : context [changed_in _ _ _] |- _ => generalize H; clear H
+        | H : Regs ?ST Rv = _  |- _ => not_eq ST s; generalize H; clear H
+        | H : context [Safe _ _ _] |- _ => not_eq H H_interp; generalize H; clear H
+      end.
+
+  Lemma Safe_Len_k_in : forall fs var ptr v k, 
+    Safe fs (Syntax.Len var ptr;: k) v ->
+    fst v[ptr] %in fst (snd v).
+    intros; eapply Safe_seq_first in H; inv_Safe_clear; eauto.
+  Qed.
+
+  Ltac simpl_interp :=
+    match goal with
+      | H: interp _ (![_](_, ?ST)), H_eval: evalInstrs _ ?ST _ = _ |- _  =>
+        simpl in H; try rewrite fold_4S in H
+    end.
+
+  Ltac pre_eval :=
+    match goal with
+      | H: interp _ (![_](_, ?ST)), H_eval: evalInstrs _ ?ST _ = _ |- _  =>
+        try clear_imports; HypothesisParty H; prep_locals; clear_bad H ST;
+          simpl_interp; simpl_sp; try rewrite fold_4S in *
+    end.
+
+  Ltac post_eval := intros; try fold (@length W) in *; post_step; try fold_length; try rewrite fold_4S in *.
+
+  Definition heap_to_split arrs (_ : W) := heap arrs.
+
+  Ltac cond_gen := try
+    match goal with
+      | H_interp : interp _ (![_](_, ?ST)), H_eval : evalInstrs _ ?ST ?INST = _ |- _ =>
+        match INST with
+          | context [variablePosition ?vars ?s] => assert_new (In s vars)
+          | context [variableSlot ?s ?vars] => assert_new (In s vars)
+          | context [ LvMem (Reg Rv) ] =>
+            match goal with
+              | H : safe_access ?ARRS ?ARR ?IDX, H_rv : Regs ST Rv = _ |- _ =>
+                assert_new (Regs ST Rv = ARR ^+ $4 ^* IDX); [ | clear H_rv; replace (heap ARRS) with (heap_tag ARRS ARR IDX) in * by eauto; set_all ARR; set_all IDX ]
+              | H : ?ARR %in fst ?ARRS, H_rv : Regs ST Rv = _ |- _ =>
+                assert_new (Regs ST Rv = ARR ^- $4); [ | clear H_rv; replace (heap ARRS) with (heap_to_split ARRS ARR) in * by eauto; set_all ARR ]
+              | H : Safe _ (Syntax.ReadAt _ ?ARR ?IDX) ?ST |- _ => eapply Safe_ReadAt_safe_access in H; simpl in H
+              | H : Safe _ (Syntax.WriteAt ?ARR ?IDX _) ?ST |- _ => eapply Safe_WriteAt_safe_access in H; simpl in H
+              | H : Safe _ (Syntax.ReadAt _ ?ARR ?IDX;: _) ?ST |- _ => generalize H; eapply Safe_ReadAt_k_safe_access in H; simpl in H
+              | H : Safe _ (Syntax.WriteAt ?ARR ?IDX _;: _) ?ST |- _ => generalize H; eapply Safe_WriteAt_k_safe_access in H; simpl in H
+              | H : Safe _ (Syntax.Len _ ?ARR;: _) ?ST |- _ => generalize H; eapply Safe_Len_k_in in H; simpl in H
+            end
+        end; [ clear H_eval .. | cond_gen ]
+    end.
+
+  Definition get_arr (arrs : arrays) addr := snd arrs addr.
+
+  Definition add_arr arrs addr ls := (fst arrs %+ addr, WDict.upd (snd arrs) addr ls).
+
+  Definition remove_arr (arrs : arrays) addr := (fst arrs %- addr, snd arrs).
+
+  Lemma star_comm : forall a b, a * b ===> b * a.
+    clear; intros; sepLemma.
+  Qed.
+
+  Lemma star_cancel_left : forall a b c, b ===> c -> a * b ===> a * c.
+    clear; intros; sepLemma.
+  Qed.
+
+  Lemma star_cancel_right : forall a b c, b ===> c -> b * a ===> c * a.
+    clear; intros; sepLemma.
+  Qed.
+
+  (* starS_equiv has been added to Sets.v. This lemma can be deleted from here after updating bedrock repo *)
+  Ltac to_himp := repeat intro.
+
+  Ltac from_himp := match goal with
+                      | [ |- interp ?specs (?p ?x ?y ---> ?q ?x ?y) ] =>
+                        generalize dependent y; generalize dependent x; generalize dependent specs;
+                          change (p ===> q)
+                    end.
+
+  Lemma starS_equiv : forall P a b, a %= b -> starS P a ===> starS P b.
+    clear.
+    intros.
+    unfold starS.
+    to_himp.
+    apply existsL.
+    intros.
+    apply existsR with x.
+    from_himp.
+    eapply star_cancel_right.
+    sepLemma.
+  Qed.
+
+  Lemma heap_equiv : forall a b, a %%= b -> heap a ===> heap b.
+    intros.
+    destruct a; destruct b.
+    unfold equiv in *.
+    simpl in H.
+    openhyp.
+    unfold heap.
+    eapply Himp_trans.
+    eapply starS_equiv.
+    eauto.
+    eapply starS_weaken.
+    intros.
+    unfold array_ptr.
+    rewrite H0.
+    eapply Himp_refl.
+    eauto.
+  Qed.
+
+  Lemma equiv_symm : forall a b, a %%= b -> b %%= a.
+    clear; unfold equiv, WMake.equiv; simpl; intros; firstorder.
+  Qed.
+
+  Hint Resolve equiv_symm.
+
+  Definition trigger A (_ : A) := True.
+
+  Lemma array_ptr_array_with_size : forall d ls p, array_ptr (WDict.upd d p ls) p = array_with_size ls p.
+    clear; intros; unfold array_ptr; rewrite WDict.sel_upd_eq; eauto.
+  Qed.
+
+  Lemma heap_bwd : forall arrs, trigger arrs -> (Ex arr_ptr, Ex old_arrs, Ex new_arr, [| arrs %%= add_arr old_arrs arr_ptr new_arr |] * [| ~ arr_ptr %in fst old_arrs |] * (heap old_arrs * array_with_size new_arr arr_ptr)) ===> heap arrs.
+    clear; intros.
+    cancel auto_ext.
+    post_step.
+    simpl in x.
+    destruct x0.
+    simpl in H1.
+    eapply Himp_trans.
+    Focus 2.
+    eapply heap_equiv.
+    eauto.
+    unfold add_arr; simpl.
+    eapply Himp_trans.
+    Focus 2.
+    eapply starS_add_bwd.
+    eauto.
+    rewrite array_ptr_array_with_size.
+    eapply Himp_trans.
+    eapply star_comm.
+    eapply star_cancel_right.
+    eapply starS_weaken.
+    intros.
+    unfold array_ptr.
+    rewrite WDict.sel_upd_ne.
+    eapply Himp_refl.
+    eauto.
+  Qed.
+
+  Ltac trigger_bwd Hprop :=
+    match Hprop with
+      context [ heap ?ARRS ] =>
+      assert (trigger ARRS) by (unfold trigger; trivial)
+    end.
+
+  Lemma equiv_refl : forall a, a %%= a.
+    clear; unfold equiv; intros; firstorder.
+  Qed.
+  Hint Resolve equiv_refl.
+
+  Hint Resolve in_not_in_ne.
+
+  Local Notation delete := Syntax.Free.
+
+  Lemma heap_fwd : forall arrs arr, arr %in fst arrs -> heap_to_split arrs arr ===> Ex new_arrs, [| new_arrs = remove_arr arrs arr |] * array_with_size (get_arr arrs arr) arr * heap new_arrs.
+    clear; intros.
+    cancel auto_ext.
+    unfold heap_to_split, heap, arrays in *.
+    destruct arrs.
+    simpl in *.
+    eapply Himp_trans.
+    eapply starS_del_fwd.
+    eauto.
+    replace (array_ptr d arr) with (array_with_size (d arr) arr) by eauto.
+    eapply star_comm.
+  Qed.
+
+  Lemma Safe_free_in : forall fs ptr v, Safe fs (delete ptr) v -> fst v [ptr] %in fst (snd v).
+    inversion 1; subst; eauto.
+  Qed.
+  Hint Resolve Safe_free_in.
+
+  Lemma RunsTo_RunsToRelax : forall fs s v1 v2,
+    fs -:- v1 -- s --> v2 ->
+    fs ~:~ v1 ~~ s ~~> v2.
+    clear; unfold RunsToRelax; intro; descend; eauto.
+  Qed.
+  Hint Resolve RunsTo_RunsToRelax.
+
+  Lemma heap_fwd_access : forall arrs arr idx, safe_access arrs arr idx -> heap_tag arrs arr idx ===> Ex new_arrs, [| new_arrs = remove_arr arrs arr |] * [| (idx < natToW (length (get_arr arrs arr)))%word |] * array_with_size (get_arr arrs arr) arr * heap new_arrs.
+    clear; intros.
+    cancel auto_ext.
+    unfold safe_access in *; simpl in *; openhyp; eauto.
+    unfold heap_tag, heap, arrays in *.
+    destruct arrs.
+    eapply Himp_trans.
+    eapply starS_del_fwd.
+    unfold safe_access in *; simpl in *; openhyp; eauto.
+    unfold get_arr; simpl.
+    replace (array_ptr d arr) with (array_with_size (d arr) arr) by eauto.
+    eapply star_comm.
+  Qed.
+
+  Lemma array_with_size_fwd : forall ls p, array_with_size ls p ===> let len := length ls in ([| p <> $8 /\ freeable (p ^- $8) (len + 2) /\ goodSize (len + 2) |] * (p ^- $8) =?> 1 * (p ^- $4) =*> natToW len * array ls p)%Sep.
+    clear; intros; unfold array_with_size; sepLemma.
+  Qed.
+
+  Lemma array_with_size_bwd : forall ls p, let len := length ls in ([| p <> $8 /\ freeable (p ^- $8) (len + 2) /\ goodSize (len + 2) |] * (p ^- $8) =?> 1 * (p ^- $4) =*> natToW len * array ls p)%Sep ===> array_with_size ls p.
+    clear; intros; unfold array_with_size; sepLemma.
+  Qed.
+
+  Definition hints_array_access_bwd : TacPackage.
+    prepare tt (heap_bwd, array_with_size_bwd).
+  Defined.
+
+  Ltac apply_save_in lemma hyp := generalize hyp; eapply lemma in hyp; intro.
+
+  Ltac assert_sp P Q H_sp :=
+    match P with
+      context [ locals _ _ _ ?P_SP ] =>
+      match Q with
+        context [ locals _ _ _ ?Q_SP] =>
+        assert (Q_SP = P_SP) as H_sp
+      end
+    end.
+
+  Ltac set_heap_goal :=
+    match goal with
+      |- context [ heap ?ARRS ] => set_all ARRS
+    end.
+
+  Ltac set_heap_hyp :=
+    match goal with
+      H : context [ heap ?ARRS ] |- _ => set_all ARRS
+    end.
+
+  Ltac set_array_hyp :=
+    match goal with
+      H : context [ array ?ARR ?PTR ] |- _ => set_all ARR; set_all PTR
+    end.
+
+  Lemma not_in_remove_arr : forall arr arrs, ~ arr %in fst (remove_arr arrs arr).
+    intros; unfold remove_arr; simpl; eauto.
+  Qed.
+
+  Hint Resolve not_in_remove_arr.
+
+  Lemma Safe_write_access : forall fs arr idx val vs arrs, 
+    Safe fs (Syntax.WriteAt arr idx val) (vs, arrs) ->
+    safe_access arrs (exprDenote arr vs) (exprDenote idx vs).
+    intros; inv_Safe_clear; eauto.
+  Qed.
+  Hint Resolve Safe_write_access.
+
+  Lemma Safe_write_k : forall fs a i e k v, let s := a[i] *<- e in Safe fs (s;: k) v -> Safe fs k (denote_sem s v).
+    clear; simpl; destruct v; inversion 1; eauto.
+  Qed.
+
+  Definition hints_heap_bwd : TacPackage.
+    prepare tt heap_bwd.
+  Defined.
+
+  Definition hints_heap_fwd : TacPackage.
+    prepare heap_fwd tt.
+  Defined.
+
+  Definition hints : TacPackage.
+    prepare (heap_fwd, heap_fwd_access, array_with_size_fwd) tt.
+  Defined.
+
+  Hint Resolve in_tran_not.
+
+  Lemma vars_require_imply : forall vars s1 s2, 
+    vars_require vars s1 -> 
+    List.incl (footprint s2) (footprint s1) ->
+    depth s2 <= depth s1 ->
+    vars_require vars s2.
+    clear; unfold vars_require; intros; openhyp; descend; eauto.
+  Qed.
+
+  Local Notation "'e_vars_require'" := CompileExpr.expr_vars_require.
+
+  Lemma vars_require_imply_e : forall vars s e base, vars_require vars s -> List.incl (varsIn e) (footprint s) -> (base + edepth e <= depth s)%nat -> e_vars_require ("__reserved" :: "__arg" :: vars) e base.
+    clear; unfold vars_require, CompileExpr.expr_vars_require; simpl; intuition; eauto.
+  Qed.
+
+  Ltac unfold_copy_vars_require :=
+    match goal with
+      H : vars_require _ _ |- _ => generalize H; unfold vars_require in H; simpl in H; intro; openhyp
+    end.
+
+  Ltac protect_hyps :=
+    repeat 
+      match goal with
+        | H : agree_except _ _ _ |- _ => generalize dependent H
+        | H : vars_require _ _ |- _ => generalize dependent H
+        | H : Regs _ Rv = _ |- _ => generalize dependent H
+        | H : safe_access _ _ _ |- _ => generalize dependent H
+        | H : _ %in _ |- _ => generalize dependent H
+        | H : Safe _ _ _ |- _ => generalize dependent H
+        | H : RunsToRelax _ _ _ _ |- _ => generalize dependent H
+      end.
+
+  Ltac step_array_access := 
+    match goal with
+      H_interp : interp ?SPECS (![?P] ?ST) |- interp ?SPECS (![?Q] ?ST) => let H_sp := fresh in 
+        assert_sp P Q H_sp; [ .. | protect_hyps; generalize H_interp H_sp; clear; intros; trigger_bwd Q; set_array_hyp; set_heap_goal; step hints_array_access_bwd; post_step ]
+    end.
+
+  Ltac changed_unchanged_disjoint :=
+    match goal with
+      H : disjoint ?A ?B |- agree_in _ _ _ => eapply changed_unchanged with (changed := B)
+    end.
+
+  Ltac changed_in_inv_disjoint := 
+    match goal with
+      H : disjoint ?A ?B |- _ = _ => eapply changed_in_inv with (vars := B)
+    end.
+
+  Ltac change_rp' :=
+    match goal with
+      H : ?SPECS (sel ?VS1 "rp") = Some _ |- ?SPECS (sel ?VS2 "rp") = Some _ =>
+        replace (sel VS2 "rp") with (sel VS1 "rp"); [ | symmetry; changed_in_inv_disjoint; [ | eapply in_tran_not; [ | eassumption ] ] ]
+    end.
+
+  Ltac equiv_solver :=
+    match goal with
+      |- _ %%= add_arr ?ARRS _ _ => auto_unfold; no_question_mark; rewriter; unfold add_arr, remove_arr, equiv; simpl; to_tempOf; split; [ | intros; repeat f_equal; erewrite changed_in_inv by eauto; rewrite sel_upd_ne by eauto; erewrite changed_in_inv by eauto; rewrite sel_upd_eq by eauto]
+    end.
+
+  Lemma Safe_read_access : forall fs var arr idx vs arrs, 
+    Safe fs (Syntax.ReadAt var arr idx) (vs, arrs) ->
+    safe_access arrs (exprDenote arr vs) (exprDenote idx vs).
+    intros; inv_Safe_clear; eauto.
+  Qed.
+  Hint Resolve Safe_read_access.
+
+  Lemma Safe_read_k : forall fs var a i k v, let s := Syntax.ReadAt var a i in Safe fs (s;: k) v -> Safe fs k (denote_sem s v).
+    clear; simpl; destruct v; inversion 1; eauto.
+  Qed.
+
+  Ltac set_vs_hyp :=
+    match goal with
+      H : context [ locals _ ?VS _ _ ] |- _ => set_all VS
+    end.
+
+  Ltac equiv_solver2 :=
+    match goal with
+      |- _ %%= add_arr ?ARRS _ _ => auto_unfold; no_question_mark; rewriter; unfold add_arr, remove_arr, equiv; simpl; to_tempOf; split; [ | intros; repeat f_equal]
+    end.
+
+  Lemma upd_sel_equiv : forall d i i', WDict.upd d i (d i) i' = d i'.
+    clear; intros; destruct (weq i i').
+    rewrite WDict.sel_upd_eq; congruence.
+    rewrite WDict.sel_upd_ne; congruence.
+  Qed.
+
+  Ltac upd_chain_solver2 :=
+    match goal with
+      H1 : changed_in _ _ _, H2 : changed_in (upd _ _ _) _ _ |- changed_in _ _ _ => no_question_mark; simpl; iter_changed
+    end.
+
+  Lemma Safe_len_in : forall fs var arr vs arrs, 
+    Safe fs (Syntax.Len var arr) (vs, arrs) ->
+    vs[arr] %in fst arrs.
+    intros; inv_Safe_clear; eauto.
+  Qed.
+  Hint Resolve Safe_len_in.
+
+  Lemma Safe_len_k : forall fs var a k v, let s := Syntax.Len var a in Safe fs (s;: k) v -> Safe fs k (denote_sem s v).
+    clear; simpl; destruct v; inversion 1; eauto.
+  Qed.
+
+  Ltac vars_require_solver :=
+    match goal with
+      | H : vars_require _ _ |- vars_require _ _ => eapply vars_require_imply; repeat (simpl; eauto)
+      | H : vars_require _ _ |- e_vars_require _ _ _ => eapply vars_require_imply_e; repeat (simpl; eauto)
+    end.
+
+  Ltac RunsToRelax_solver :=
+    match goal with
+      H : _ ~:~ _ ~~ ?S ~~> ?ST |- _ ~:~ _ ~~ ?S ~~> ?ST =>
+        eapply RunsToRelax_immune; [ eassumption | unfold st_agree_except; repeat split .. | ]
+    end.
+
+  Ltac Safe_cond_solver :=
+    match goal with
+      H : Safe _ (If _ _ _;: _) (?ST1, _) |- Safe _ _ _ =>
+        eapply Safe_immune with (vs1 := ST1); [ | use_changed_unchanged; simpl; eapply disjoint_trans_lr]
+    end.
+
+  Ltac RunsToRelax_seq_solver :=
+    match goal with
+      H : _ ~:~ _ ~~ _;: (_;: _) ~~> _ |- _ ~:~ _ ~~ _;: _;: _ ~~> _ =>
+        eapply RunsToRelax_assoc_left; simpl
+    end.
+
+  Ltac rv_solver' :=
+    match goal with
+      | H:Regs ?ST Rv = _ |- Regs ?ST Rv = _ => pattern_l; rewriter
+      | H:Regs ?ST Rv = _ |- _ = Regs ?ST Rv => pattern_r; rewriter
+      | H:_ = Regs ?ST Rv |- Regs ?ST Rv = _ => pattern_l; rewriter_r
+      | H:_ = Regs ?ST Rv |- _ = Regs ?ST Rv => pattern_r; rewriter_r
+    end.
+
+  Ltac RunsToRelax_assign_solver :=
+    match goal with
+      H : _ ~:~ _ ~~ ?K ~~> _ |- _ ~:~ _ ~~ _ <- _;: ?K ~~> _ =>
+        eapply RunsToRelax_assign; [ eassumption | unfold st_agree_except | ]; simpl
+    end.
+
+  Ltac Safe_assign_solver :=
+    match goal with
+      H : Safe _ (_ <- _;: ?K) _ |- Safe _ ?K _ =>
+        eapply Safe_immune; [ eapply Safe_assign; eassumption | eapply changed_unchanged; [ rewriter; use_changed_in_upd_same | ] ]
+    end.
+
+  Ltac rp_upd_solver :=
+    match goal with
+      |- ?A = Some _ =>
+      match A with
+        context [ upd ] =>
+        match A with
+          context [ "rp" ] =>
+          rewrite sel_upd_ne; [ change_rp' | eapply in_not_in_ne ]
+        end
+      end
+    end.
+
+  Local Notation agree_except_symm := changedVariables_symm.
+
+  Ltac RunsToRelax_Stuff_solver :=
+    eapply RunsToRelax_seq_bwd; [ | eassumption | eauto ];
+      eapply RunsToRelax_immune; [ eapply RunsTo_RunsToRelax; econstructor; eauto | .. ];
+        [ | unfold st_agree_except; repeat split; simpl | ];
+        unfold st_agree_except; simpl; intuition eauto.
+
+  Ltac do_RunsToRelax_Read_Write_solver := eapply RunsToRelax_seq_bwd; [ | eassumption | ..]; [ eapply RunsToRelax_immune; [ eapply RunsTo_RunsToRelax; econstructor; eauto | .. ]; [ | unfold st_agree_except; repeat split; simpl; eapply agree_except_symm | ] | ].
+
+  Ltac RunsToRelax_Read_Write_solver :=
+    match goal with
+      | |- _ ~:~ _ ~~ _ [ _ ] *<- _;: _ ~~> _ => do_RunsToRelax_Read_Write_solver
+      | |- _ ~:~ _ ~~ Syntax.ReadAt _ _ _;: _ ~~> _ => do_RunsToRelax_Read_Write_solver
+      | |- _ ~:~ _ ~~ Syntax.Len _ _;: _ ~~> _ => do_RunsToRelax_Read_Write_solver
+    end.
+
+  Ltac freeable_goodSize_solver :=
+    match goal with
+      | |- freeable _ _ => auto_unfold; rewrite upd_length in *
+      | |- goodSize _ => auto_unfold; rewrite upd_length in *
+    end.
+
+  Ltac himp_length_solver :=
+    match goal with
+      |- (himp _ (_ =*> natToW (length ?A)) (_ =*> natToW (length ?B)))%Sep =>
+      unfold B; repeat hiding ltac:(step hints_array_access_bwd)
+    end.
+
+  Ltac equiv_solver2' :=
+    match goal with
+      |- _ %%= add_arr _ _ _ =>
+      equiv_solver2; [ | unfold get_arr; symmetry; eapply upd_sel_equiv ]
+    end.
+
+  Ltac pick_Safe := 
+    match goal with
+      | H : Safe _ (_ [ _ ] *<- _;: ?K) _ |- Safe _ ?K _ =>
+        eapply Safe_write_k in H; eapply Safe_immune; [ eassumption | ]
+      | H : Safe _ (Syntax.ReadAt _ _ _;: ?K) _ |- Safe _ ?K _ =>    
+        eapply Safe_read_k in H; eapply Safe_immune; [ eassumption | ]
+      | H : Safe _ (Syntax.Len _ _;: ?K) _ |- Safe _ ?K _ =>    
+        eapply Safe_len_k in H; eapply Safe_immune; [ eassumption | ]
+      | H : Safe _ (Syntax.Assignment _ _;: ?K) _ |- Safe _ ?K _ =>    
+        eapply Safe_assign in H; eapply Safe_immune; [ eassumption | ]
+    end.
+
+  Ltac pre_eauto := try first [
+    use_disjoint_trans' |
+    use_Safe_immune2 |
+    extend_runs_loop_partially |
+    use_changed_in_eval |
+    arrays_eq_solver |
+    format_solver |
+    use_changed_in_upd_same |
+    not_in_solver |
+    equiv_solver |
+    upd_chain_solver |
+    arrays_eq_solver2 |
+    RunsTo_Malloc
+    ].
+
+  Lemma mult_S_distr_inv : forall a b, a + a * b = a * S b.
+    intros; ring.
+  Qed.
+
+  Lemma wplus_wminus : forall (a b : W), a ^+ b ^- b = a.
+    intros; words.
+  Qed.
+
+  Ltac rewrite_expr :=
+    match goal with
+      | H : context [exprDenote ?E ?VS1] |- context [exprDenote ?E ?VS2] => not_eq VS1 VS2; rewrite (@unchanged_exprDenote _ VS1 VS2)
+    end.
+
+  Ltac change_locals ns' avail' :=
+    match goal with
+      H : context[locals ?ns ?vs ?avail ?p] |- _ =>
+        let offset := eval simpl in (4 * List.length ns) in
+          change (locals ns vs avail p) with (locals_call ns vs avail p ns' avail' offset) in H; assert (ok_call ns ns' avail avail' offset)%nat
+    end.
+
+  Ltac change_sp :=
+    match goal with
+      Hinterp : interp _ (![ ?P ] (_, ?ST)), Heval : evalInstrs _ ?ST _ = _ |- _ =>
+        match P with
+          context [ Regs ?ST2 Sp ] => not_eq ST ST2; replace (Regs ST2 Sp) with (Regs ST Sp) in Hinterp by words
+        end
+    end.
+
+  Ltac generalize_sp :=
+    repeat match goal with
+             H : Regs _ Sp = Regs _ Sp |- _ => generalize dependent H
+           end.
+
+  Ltac agree_in_solver :=
+    match goal with
+      |- agree_in _ _ _ => changed_unchanged_disjoint; [ iter_changed; incl_app_solver | .. ]
+    end.
+
+  Ltac use_Safe_immune' :=
+    match goal with
+      H : Safe _ ?S (_, ?A) |- Safe _ ?S (_, ?A) =>
+        eapply Safe_immune; [ eassumption | .. ]; agree_in_solver
+    end.
+
+  Ltac ok_call_solver :=
+    match goal with
+      |- ok_call _ _ _ _ _ =>
+      repeat split; simpl; unfold MIN_RESERVED in *; eauto; NoDup
+    end.
+
+  Ltac myPost := autorewrite with sepFormula in *; unfold substH in *; simpl in *.
+
+  Lemma aug_rp_not_in : forall vars, ~ In "rp" vars -> ~ In "rp" ("__reserved" :: "__arg" :: vars).
+    simpl; intuition.
+  Qed.
+
+  Ltac prep_rp :=
+    match goal with 
+      H : ~ In "rp" ?VARS |- _ =>
+        match VARS with
+          | context ["__reserved"] => fail 1
+          | _ => eapply aug_rp_not_in in H
+        end
+    end.
+
+  Hint Resolve heap_star_not_in.
+
+  Ltac rearrange_heap :=
+    match goal with
+      H : interp ?SPECS (![?P] ?ST) |- _ =>
+        match P with
+          context [ heap ?ARRS ] =>
+          match P with 
+            context [ array_with_size ?LS ?PTR ] =>
+            rearrange_stars (heap ARRS * array_with_size LS PTR)%Sep
+          end
+        end
+    end.
+
+  Lemma not_in_reserved_arg : forall vars, ~ In "__reserved" vars -> ~ In "__reserved" ("__arg" :: vars).
+    simpl; intuition.
+  Qed.
+
+  Hint Resolve not_in_reserved_arg.
+
+  Lemma Safe_Malloc_goodSize : forall fs var size v, Safe fs (Syntax.Malloc var size) v -> let size_v := exprDenote size (fst v) in goodSize (wordToNat size_v + 2).
+    inversion 1; subst; eauto.
+  Qed.
+
+  Hint Resolve Safe_Malloc_goodSize.
+
+  Lemma Safe_malloc_goodSize : forall fs var size vs arrs, Safe fs (Syntax.Malloc var size) (vs, arrs) -> let size_v := exprDenote size vs in goodSize (wordToNat size_v + 2).
+    intros; eapply (@Safe_Malloc_goodSize _ _ _ (vs, arrs)); eauto.
+  Qed.
+
+  Hint Resolve Safe_malloc_goodSize.
+
+  Ltac clear_or :=
+    repeat match goal with 
+             H : _ \/ _ |- _ => clear H 
+           end.
+
+  Ltac simpl_vars :=
+    repeat match goal with 
+             | H : context [footprint _] |- _ => progress simpl in H
+             | H : context [tmps _] |- _ => progress simpl in H
+           end.
+
+  Ltac tempOf_in_ext_solver :=
+    match goal with
+      |- In (tempOf _) ("__reserved" :: "__arg" :: ?VARS) =>
+      eapply In_incl with (ls1 := VARS)
+    end.
+
+  Ltac replace_reserved :=
+    match goal with
+      H : context [sel ?VS1 "__reserved"] |- context [sel ?VS2 "__reserved"] =>
+        not_eq VS1 VS2; replace (sel VS2 "__reserved") with (sel VS1 "__reserved") in *
+    end.
+
+  Lemma ignore_premise : forall pc state specs (P Q : PropX pc state),
+    interp specs Q
+    -> interp specs (P ---> Q).
+    intros; apply Imply_I; apply interp_weaken; assumption.
+  Qed.
+
+  Ltac step_himp_helper :=
+    match goal with
+      |- himp _ ?A ?B =>
+      match B with
+        context [locals ?VARS ?VS1 _ ?SP1] =>
+        match A with
+          context [locals VARS ?VS2 _ ?SP2] =>
+          match A with
+            context [locals ?VARS2 _ _ ?SP3] =>
+            not_eq VARS VARS2; replace SP1 with SP2; replace SP3 with (SP2 ^+ natToW (4 * length VARS)); replace VS1 with VS2
+          end
+        end
+      end
+    end.
+
+  Ltac sel_eq_solver :=
+    match goal with
+      |- sel _ ?V = sel _ ?V => symmetry; changed_in_inv_disjoint
+    end.
+
+  Ltac pre_eauto2 := try first [
+    ok_call_solver |
+    use_Safe_immune2 |
+    (format_solver; incl_app_solver) |
+    equiv_solver |
+    vars_require_solver |
+    RunsToRelax_solver | 
+    rp_upd_solver |
+    change_rp' |
+    rv_solver' |
+    Safe_cond_solver |
+    RunsToRelax_seq_solver |
+    RunsToRelax_assign_solver |
+    Safe_assign_solver | 
+    RunsToRelax_Read_Write_solver |
+    freeable_goodSize_solver |
+    changed_unchanged_disjoint |
+    himp_length_solver |
+    equiv_solver2' |
+    use_Safe_immune' |
+    sel_eq_solver |
+    tempOf_in_ext_solver
+    ].
+
+  Lemma four_out : forall n, 4 * (S (S (S n))) = 4 * 3 + 4 * n.
+    intros; omega.
+  Qed.
+
+  Ltac eval_instrs hints :=
+    match goal with
+      | H: interp _ (![_](_, ?ST)), H_eval: evalInstrs _ ?ST _ = _ |- _  =>
+        cond_gen; [ .. | let P := fresh "P" in
+          try match goal with
+                | [ _ : context[Safe ?fs _ _] |- _ ] => set (P := Safe fs) in *
+              end;
+          pre_eval;
+          try match goal with
+                | [ H : _ = Regs ?X Rv, H' : _ = Regs ?X Rv |- _ ] => generalize dependent H'
+              end;
+          my_evaluate hints;
+          try subst P;
+            post_eval; clear H_eval]
+    end.
+
+  Ltac clear_specs :=
+    repeat
+      match goal with
+        | H : interp ?SPECS_H _ |- context [simplify ?SPECS _ _] => not_eq SPECS_H SPECS; clear H
+        | H : interp ?SPECS_H _ |- context [interp ?SPECS _] => not_eq SPECS_H SPECS; clear H
+      end.
+
+  Ltac pre_eval_statement := intros; open_hyp; try_post.
+
+  Ltac eval_statement := pre_eval_statement; transit; open_hyp; try_post.
+
+  Ltac eval_step hints := first[eval_statement | try clear_imports; eval_instrs hints].
+
+  Local Notation skip := Syntax.Skip.
 
   Lemma Safe_skip : forall fs k v a,
     Safe fs (skip;: k) (v, a)
@@ -260,7 +1943,7 @@ Section Compiler.
   Hint Extern 1 (agree_in _ _ _) => progress simpl.
 
   Lemma Safe_loop_false : forall fs e b v k,
-    Safe fs (Loop e b;: k) v ->
+    Safe fs (While e b;: k) v ->
     wneb (v[(e)]) $0 = false ->
     Safe fs k v.
     intros; inv_Safe; eauto.
@@ -315,13 +1998,13 @@ Section Compiler.
 
   Ltac Safe_cond_solver :=
     match goal with
-      H : Safe _ (Conditional _ _ _;: _) (?ST1, _) |- Safe _ _ _ =>
+      H : Safe _ (If _ _ _;: _) (?ST1, _) |- Safe _ _ _ =>
         eapply Safe_immune with (vs1 := ST1); [ decide_cond_safe | use_changed_unchanged; simpl; eapply disjoint_trans_lr]
     end.
 
   Ltac Safe_loop_solver :=
     match goal with
-      |- Safe _ (_ ;: (Loop _ _ ;: _)) _ => decide_cond ltac:(eapply Safe_loop_true_k) ltac:(eapply Safe_loop_false)
+      |- Safe _ (_ ;: (While _ _ ;: _)) _ => decide_cond ltac:(eapply Safe_loop_true_k) ltac:(eapply Safe_loop_false)
     end.
 
   Ltac pre_eauto2 := try first [
@@ -382,6 +2065,8 @@ Section Compiler.
           context [ locals _ ?VS _ _ ] => let a := fresh in evar (a : arrays); (exists (VS, a)); unfold a in *; clear a
         end
     end.
+
+  Ltac unfold_eval := unfold precond, postcond, inv, expr_runs_to, runs_to_generic, vars, MIN_RESERVED in *.
 
   Ltac preamble := 
     wrap0; unfold_eval; unfold_copy_vars_require; myPost;
@@ -1044,2193 +2729,4 @@ Section Compiler.
   Definition statementCmd (s k : Statement) := Wrap imports imports_global modName (compile s k) (fun _ => postcond k) (verifCond s k imports) (@post_ok s k) (@verifCond_ok s k).
 
 End Compiler.
-Definition array_ptr lists p : HProp := array_with_size (lists p) p.
-
-Lemma star_diff_ptrs : forall specs st other p1 p2, interp specs (![p1 =?>1 * p2 =?> 1 * other] st) -> p1 <> p2.
-  rewrite sepFormula_eq.
-  propxFo.
-  subst.
-  unfold smem_get_word in *.
-  simpl in *.
-  case_eq (smem_get p2 x3).
-  intros.
-  clear H6.
-  case_eq (smem_get p2 x6).
-  clear H9.
-  intros.
-  destruct H2.
-  subst.
-  destruct H5.
-  subst.
-  destruct H4.
-  subst.
-  Require Import Bootstrap.
-  eapply disjoint_get_fwd in H2.
-  eauto.
-  erewrite join_Some by eassumption.
-  discriminate.
-  erewrite join_Some by eassumption.
-  discriminate.
-  intros.
-  rewrite H0 in H9.
-  discriminate.
-  intros.
-  rewrite H in H6.
-  discriminate.
-Qed.
-
-Hint Resolve star_diff_ptrs.
-
-Ltac hiding tac :=
-  (let P := fresh "P" in
-    match goal with
-      | [ H : Safe ?fs _ _ |- _ ] => set (P := Safe fs) in *
-      | [ H : ?fs ~:~ _ ~~ _ ~~> _ |- _ ] => set (P := RunsToRelax fs) in *
-    end;
-    hiding tac;
-    subst P) || tac.
-
-Ltac rearrange_stars HEAD :=
-  match goal with
-    H : interp ?SPECS (![?P] ?ST) |- _ =>
-      let OTHER := fresh in 
-        evar (OTHER : HProp); 
-        assert (interp SPECS (![HEAD * OTHER] ST));
-          unfold OTHER in *; clear OTHER;
-            [ hiding ltac:(step auto_ext) | .. ]
-  end.
-
-Infix "=~*>" := (ptsto32 nil) (at level 30).
-
-Lemma array_with_size_star_diff : forall specs st other ls1 p1 ls2 p2, interp specs (![array_with_size ls1 p1 * array_with_size ls2 p2 * other] st) -> p1 <> p2.
-  unfold array_with_size; intros.
-  rearrange_stars ((p1 ^- $ (8)) =?> 1 * (p2 ^- $ (8)) =?> 1)%Sep; eauto.
-  eapply star_diff_ptrs in H1.
-  intuition.
-Qed.
-
-Hint Resolve array_with_size_star_diff.
-
-Lemma starS_not_in : forall specs st d ptrs ls p other, interp specs (![starS (array_ptr d) ptrs * array_with_size ls p * other] st) -> ~ p %in ptrs.
-  intros.
-  intro.
-  assert (interp specs
-        (![(starS (array_ptr d) (ptrs %- p) * array_ptr d p) * array_with_size ls p * other] st)).
-  set (starS (array_ptr d) ptrs) in *.
-  set (starS (array_ptr d) (ptrs %- p)) in *.
-  set (array_with_size ls p) in *.
-  set (array_ptr d p) in *.
-  step auto_ext.
-  unfold h, h0, h2.
-  eapply Himp_trans.
-  eapply starS_del_fwd.
-  eauto.
-  set (starS (array_ptr d) (ptrs %- p)) in *.
-  set (array_ptr d p) in *.
-  sepLemma.
-  clear H.
-  unfold array_ptr in H1 at 2.
-  set (starS (array_ptr d) (ptrs %- p)) in *.
-  rearrange_stars (array_with_size (d p) p * array_with_size ls p)%Sep.
-  eapply array_with_size_star_diff in H2.
-  intuition.
-Qed.
-
-Lemma heap_star_not_in : forall specs st other arrs ls p, interp specs (![heap arrs * array_with_size ls p * other] st) -> ~ p %in fst arrs.
-  intros; unfold arrays in *; destruct arrs; unfold heap in *; simpl in *; eapply starS_not_in; eauto.
-Qed.
-
-Ltac auto_apply :=
-  match goal with
-    H : _ |- _ => eapply H
-  end.
-
-Ltac open_Some := 
-  match goal with
-    H : Some _ = Some _ |- _ => injection H; clear H; intros
-  end.
-
-Ltac condition_solver :=  
-  match goal with
-    H : evalCond _ _ _ _ _ = Some ?T |- wneb _ _ = ?T => 
-    unfold evalCond in *; simpl in *; open_Some; rewriter_r; f_equal
-  end.
-
-Local Notation "var <- 'new' size" := (Syntax.Malloc var size) (no associativity, at level 60).
-
-Open Scope nat.
-
-Hint Rewrite sum_S : arith.
-Hint Resolve S_le_lt.
-Hint Resolve sel_upd_firstn.
-Hint Resolve firstn_S_upd.
-Hint Resolve VariableLemmas.noChange.
-Hint Resolve Max.le_max_l Max.le_max_r.
-Hint Extern 12 => rv_solver.
-Hint Extern 12 => sp_solver.
-Hint Resolve le_plus_lt lt_max_l lt_max_r.
-Hint Resolve plus_le.
-Hint Resolve lt_le_S plus_lt.
-
-Lemma le_max_l_trans : forall a b c, (a <= b -> a <= max b c)%nat.
-  intros; eapply le_trans.
-  2: eapply Max.le_max_l.
-  eauto.
-Qed.
-Hint Resolve le_max_l_trans.
-
-Lemma le_max_r_trans : forall a b c, (a <= c -> a <= max b c)%nat.
-  intros; eapply le_trans.
-  2: eapply Max.le_max_r.
-  eauto.
-Qed.
-Hint Resolve le_max_r_trans.
-
-Ltac max_le_solver :=
-  repeat 
-    match goal with
-      | |- ?A <= ?A => eapply le_n
-      | |- max ?A ?B <= _ => eapply Max.max_lub
-      | |- ?S <= max ?A _ =>
-        match A with
-          context [ S ] => eapply le_max_l_trans
-        end
-      | |- ?S <= max _ ?B =>
-        match B with
-          context [ S ] => eapply le_max_r_trans
-        end
-    end.
-Hint Extern 0 (_ <= _) => progress max_le_solver.
-
-Ltac incl_app_solver :=
-  repeat 
-    match goal with
-      | |- List.incl ?A ?A => eapply List.incl_refl
-      | |- List.incl (?A ++ ?B) _ => eapply incl_app
-      | |- List.incl (?A :: ?B) _ => eapply List.incl_cons
-      | |- List.incl ?S (?A ++ _) =>
-        match A with
-          context [ S ] => eapply incl_appl
-        end
-      | |- List.incl ?S (_ ++ ?B) =>
-        match B with
-          context [ S ] => eapply incl_appr
-        end
-      | |- List.incl ?S (?A :: _) =>
-        match A with
-          context [ S ] => eapply (@incl_appl _ _ _ (_ :: nil))
-        end
-      | |- List.incl ?S (?A :: ?B) =>
-        match B with
-          context [ S ] => eapply (@incl_appr _ _ (_ :: nil))
-        end
-    end.
-Hint Extern 0 (List.incl _ _) => progress incl_app_solver.
-
-Hint Resolve in_eq In_incl.
-Hint Resolve List.incl_cons incl_cons_l incl_cons_r List.incl_refl incl_nil incl_tl incl_array.
-Hint Resolve incl_app incl_appl incl_appr.
-Hint Resolve List.incl_tran.
-Hint Resolve disjoint_trans_lr.
-Hint Resolve changedVariables_upd.
-Hint Resolve unchanged_in_except_disjoint unchanged_in_except_upd unchanged_in_except_shrink.
-Hint Constructors or.
-Hint Resolve sel_upd_eq.
-
-Hint Constructors RunsTo.
-Hint Constructors runs_loop_partially.
-Hint Resolve unchanged_exprDenote.
-Hint Resolve changedVariables_upd_bwd.
-Hint Resolve unchanged_incl.
-Hint Resolve two_merge_equiv.
-Hint Resolve changed_in_upd_same.
-
-Hint Extern 12 (unchanged_in _ _ _) => use_changed_unchanged.
-Hint Extern 12 (unchanged_in _ _ _) => use_changed_unchanged'.
-Hint Extern 12 (changed_in _ _ _) => use_changed_trans2.
-Hint Extern 12 (changed_in _ _ _) => use_changed_incl.
-Hint Extern 12 => condition_solver'.
-Hint Extern 12 (unchanged_in _ _ _) => use_unchanged_in_symm.
-Hint Extern 12 (changed_in _ _ _) => use_changed_in_symm.
-
-Hint Resolve runs_loop_partially_finish.
-Hint Resolve exprDenote_disjoint.
-Hint Resolve RunsTo_footprint.
-
-Hint Extern 12 (_ = _) => condition_solver.
-
-Ltac use_unchanged_exprDenote :=
-  match goal with
-    |- exprDenote ?E _ = exprDenote ?E _ => eapply unchanged_exprDenote; solve [eauto]
-  end.
-Hint Extern 12 => use_unchanged_exprDenote.
-
-Lemma incl_tempChunk2 : forall b n m, b + n <= m -> List.incl (tempChunk b n) (tempVars m).
-  intros; eapply incl_tempChunk; eauto.
-Qed.
-
-Hint Resolve incl_tempChunk2.
-
-Ltac auto_apply_in t :=
-  match goal with
-    H : _ |- _ => eapply t in H
-  end.
-
-Ltac apply_in_all t :=
-  repeat match goal with
-           H : _ |- _ => eapply t in H
-         end.
-
-Ltac inv_Safe :=
-  match goal with
-    H : Safe _ _ _ |- _ => inversion H
-  end.
-
-Ltac break_st := unfold st in *; repeat break_pair; simpl in *.
-
-Ltac use_Safe_immune :=
-  match goal with
-    H : RunsTo _ _ _ _, H2 : context [RunsTo _ _ _ _ -> Safe _ _ _] |- _ => eapply H2 in H; break_st; eapply Safe_immune
-  end.
-
-Ltac change_RunsTo :=
-  match goal with
-    H : RunsTo _ _ (?VS1, ?ARRS) _, H2 : changed_in ?VS2 ?VS1 _ |- _ => 
-      generalize H; eapply RunsTo_immune with (vs1' := (VS2, ARRS)) in H; intros
-  end.
-
-Definition equiv (a b : arrays) := fst a %= fst b /\ forall e, e %in fst a -> snd a e = snd b e.
-
-Infix "%%=" := equiv (at level 70, no associativity).
-
-Lemma disjoint_cons : forall A a (e : A) b, ~In e a -> disjoint a b -> disjoint a (e :: b).
-  unfold disj; intros; simpl; intuition; eauto.
-Qed.
-
-Lemma disjoint_disj : forall A (a : list A) b, disjoint a b -> disj a b.
-  unfold disj, disj; eauto.
-Qed.
-
-Lemma changed_trans_l : forall vs1 vs2 vs3 a c, 
-  changedVariables vs1 vs2 a -> 
-  changedVariables vs2 vs3 c ->
-  List.incl a c ->
-  changedVariables vs1 vs3 c.
-  eauto.
-Qed.
-
-Lemma del_not_in : forall s e, ~ e %in s %- e.
-  unfold mem, del; intros; intuition.
-Qed.
-
-Ltac is_reg t r :=
-  match t with
-    | _ # r => idtac
-    | Regs _ r => idtac
-  end.
-
-Ltac sp_solver' := 
-  match goal with
-    |- ?A = ?B => is_reg A Sp; is_reg B Sp; pattern_r; rewriter_r
-  end.
-
-Hint Extern 12 => sp_solver'.
-
-Ltac use_disjoint_trans :=
-  match goal with
-    H : disjoint ?A ?B |- disjoint ?C _ =>
-      match A with context [ C ] =>
-        eapply (@disjoint_trans_lr _ A B C _ H); [ | eapply List.incl_refl ]
-      end 
-  end.
-
-Hint Resolve del_not_in.
-Hint Resolve temp_in_array.
-Hint Resolve temps_not_in_array.
-Hint Resolve true_false_contradict.
-
-Ltac to_tempOf :=
-  replace "!." with (tempOf 1) in * by eauto;
-    replace "." with (tempOf 0) in * by eauto.
-
-Lemma del_add : forall s e, e %in s -> s %- e %+ e %= s.
-  clear; intros.
-  set (s %- e).
-  eapply WMake.equiv_symm.
-  eapply del_to_add.
-  eauto.
-  unfold s0; eauto.
-Qed.
-
-Hint Resolve le_n_S.
-
-Ltac use_disjoint_trans' :=
-  match goal with
-    H : disjoint ?A ?B |- disjoint ?C _ =>
-      match A with context [ C ] =>
-        eapply (@disjoint_trans_lr _ A B C _ H)
-      end 
-  end.
-
-Hint Resolve Safe_cond_true Safe_cond_false.
-
-Ltac decide_constructor :=
-  match goal with
-    H : evalCond _ _ _ _ _ = Some ?B |- RunsTo (Syntax.Conditional _ _ _) _ _ =>
-      match B with
-        | true => econstructor 6
-        | false => econstructor 7
-      end
-  end.
-
-Hint Extern 1 => decide_constructor.
-
-Hint Resolve runs_loop_partially_body_safe.
-
-Hint Resolve Safe_immune.
-
-Ltac tempOf_solver :=
-  match goal with
-    H : List.incl (tempVars _) ?VARS |- In (tempOf ?N) ?VARS =>
-      eapply In_incl; [eapply temp_in_array with (n := S N); omega | eapply incl_tran with (2 := H) ]
-  end.
-
-Hint Extern 1 => tempOf_solver.
-
-Opaque tempVars.
-
-Ltac incl_tran_tempVars :=
-  match goal with
-    H : List.incl (tempVars _) ?VARS |- List.incl (tempVars _) ?VARS => eapply incl_tran with (2 := H)
-  end.
-
-Hint Extern 1 => incl_tran_tempVars.
-
-Ltac clear_step := try clear_imports; step auto_ext.
-
-Ltac in_solver :=
-  match goal with
-    H : Safe _ _ (_, ?ARRS) |- _ %in fst ?ARRS => rewriter; inv_Safe
-  end.
-
-Hint Extern 1 => in_solver.
-
-Ltac use_Safe_immune2 :=
-  match goal with
-    | H : Safe _ ?S_H (?VS1, ?ARRS), H2 : changed_in ?VS1 ?VS2 _ |- Safe _ ?S_G (?VS2, ?ARRS) =>
-      match S_H with
-        context [ S_G ] => eapply (@Safe_immune _ S_G VS1 VS2 ARRS); [ | simpl; use_changed_unchanged; use_disjoint_trans']
-      end
-    | H : Safe _ (Syntax.Seq ?A ?B) ?V, H2 : RunsTo _ ?A ?V ?V' |- Safe _ ?B _ => break_st; rewriter; eapply Safe_immune
-    | H : Safe _ (Loop ?E ?B) _, H2 : runs_loop_partially ?E ?B _ _ |- Safe _ ?B _ => break_st; rewriter; eapply Safe_immune; [ eapply (@runs_loop_partially_body_safe _ _ _ _ _ H2) | ]; [ try use_Safe_immune2 | .. ]
-  end.
-
-Lemma Safe_seq_first : forall fs a b v, Safe fs (Syntax.Seq a b) v -> Safe fs a v.
-  intros; inv_Safe; eauto.
-Qed.
-
-Hint Resolve Safe_seq_first.
-
-Lemma unchanged_in_refl : forall vs vars, unchanged_in vs vs vars.
-  unfold unchanged_in; eauto.
-Qed.
-
-Hint Resolve unchanged_in_refl.
-
-Lemma Safe_seq_second : forall fs a b v v', Safe fs (Syntax.Seq a b) v -> RunsTo fs a v v' -> Safe fs b v'.
-  intros; inv_Safe; use_Safe_immune; eauto.
-Qed.
-
-Hint Resolve Safe_seq_second.
-
-Ltac change_RunsTo_arrs :=
-  match goal with
-    H : RunsTo _ ?S (?VS, ?ARRS1) _ |- RunsTo _ ?S (?VS, ?ARRS2) _ => replace ARRS2 with ARRS1
-  end.
-
-Hint Extern 1 => change_RunsTo_arrs.
-
-Ltac extend_runs_loop_partially :=
-  match goal with
-    H : runs_loop_partially _ ?E ?B ?V (?VS, _), H2 : RunsTo _ ?B (?VS, _) ?V'' |- runs_loop_partially _ ?E ?B ?V _ =>
-      eapply (@LoopPartialStep _ _ _ _ _ V'' H)
-  end.
-
-Ltac use_changed_in_eval :=
-  match goal with
-    H : VariableLemmas.equiv ?V (merge _ _ _) |- changed_in ?V _ _ =>
-      apply_in_all RunsTo_footprint; eapply changed_in_eval; [eassumption | ..]
-  end.
-
-Ltac pre_descend := first [change_RunsTo | auto_apply_in runs_loop_partially_finish; [change_RunsTo | ..] ]; open_hyp; break_st.
-
-Ltac arrays_eq_solver :=
-  match goal with
-    |- ?A = _ =>
-    match type of A with
-      arrays => simpl in *; congruence
-    end
-  end.
-
-Ltac choose_changed_unchanged :=
-  match goal with
-    H : disjoint ?A ?B |- unchanged_in _ _ ?C =>
-      match A with
-        context [ C ] => eapply (@changed_unchanged _ _ B _)
-      end
-  end.
-
-Ltac iter_changed_discharger := first [eassumption | eapply changedVariables_incl; [eassumption | ..] | eapply changedVariables_upd_fwd | eapply changedVariables_incl; [eapply changedVariables_upd_fwd | ..] ].
-
-Ltac iter_changed := repeat first [iter_changed_discharger | eapply changed_trans_l].
-
-Ltac format_solver :=
-  match goal with
-    |- _ = exprDenote _ _ ^+ $4 ^* exprDenote _ _ =>
-    rewriter; erewrite changed_in_inv by eauto; rewrite sel_upd_eq by eauto; rewriter; repeat (f_equal; try (eapply unchanged_exprDenote; choose_changed_unchanged; iter_changed))
-  end.
-
-Opaque List.incl.
-
-Lemma changed_in_upd_eq : forall vs1 vs2 vars s val1 val2,
-  changed_in vs1 vs2 vars ->
-  val2 = val1 ->
-  changed_in (upd vs1 s val1) (upd vs2 s val2) vars.
-  intros; rewriter; eauto.
-Qed.
-
-Hint Resolve changed_in_upd_eq.
-
-Lemma safe_access_in : forall arrs arr idx, safe_access arrs arr idx -> arr %in fst arrs.
-  unfold safe_access; intuition.
-Qed.
-
-Hint Resolve safe_access_in.
-
-Ltac use_changed_in_upd_same :=
-  match goal with
-    |- changed_in (upd _ ?S _) (upd _ ?S _) _ => eapply changed_in_upd_same; iter_changed
-  end.
-
-Ltac auto_unfold :=
-  repeat match goal with
-           t := _ |- _ => unfold t in *; clear t
-         end.
-
-Hint Resolve del_add.
-
-Hint Resolve WMake.equiv_symm.
-
-Ltac max_2_plus :=
-  match goal with
-    |- (max _ _ >= 2 + _)%nat => simpl
-  end.
-
-Hint Extern 1 => max_2_plus.
-
-Ltac tempOf_neq :=
-  match goal with
-    |- ~ (tempOf _ = tempOf _) => discriminate
-  end.
-
-Hint Extern 1 => tempOf_neq.
-
-Ltac not_in_solver :=
-  match goal with 
-    H : ?ARRS = _ |- ~ _ %in fst ?ARRS => rewriter
-  end.
-
-Ltac no_question_mark :=
-  match goal with
-    |- ?T => match T with T => idtac end
-  end.
-
-Ltac upd_chain_solver :=
-  match goal with
-    H1 : changed_in _ _ _, H2 : changed_in (upd _ _ _) _ _, H3 : changed_in (upd _ _ _) _ _ |- changed_in _ _ _ => no_question_mark; simpl; iter_changed
-  end.
-
-Ltac rv_length_solver :=
-  match goal with
-    H : Regs ?ST Rv = natToW (length _) |- Regs ?ST Rv = natToW (length _) => rewriter
-  end.
-
-Hint Extern 1 => rv_length_solver.
-
-Ltac arrays_eq_solver2 :=
-  match goal with
-    H : ?A = _ |- ?A = _ =>
-      match type of A with
-        arrays => rewriter
-      end
-  end.
-
-Ltac RunsTo_Malloc :=
-  match goal with
-    |- RunsTo _ (Syntax.Malloc _ _) _ _ => econstructor
-  end.
-
-Lemma RunsToRelax_loop_false : forall fs e b k v1 v2, 
-  fs ~:~ v1 ~~ k ~~> v2 -> 
-  wneb (v1[(e)]) $0 = false -> 
-  fs ~:~ v1 ~~ Loop e b;: k ~~> v2.
-  unfold RunsToRelax; intros; openhyp; descend; eauto.
-Qed.
-Hint Resolve RunsToRelax_loop_false.
-
-Hint Constructors Safe.
-Lemma Safe_cond_true_k : forall fs e t f k v, 
-  Safe fs (Conditional e t f;: k) v ->
-  wneb (v[(e)]) $0 = true ->
-  Safe fs (t;: k) v.
-  inversion 1; intros; econstructor; eauto.
-Qed.
-Hint Resolve Safe_cond_true_k.
-Lemma Safe_cond_false_k : forall fs e t f k v, 
-  Safe fs (Conditional e t f;: k) v ->
-  wneb (v[(e)]) $0 = false ->
-  Safe fs (f;: k) v.
-  inversion 1; intros; econstructor; eauto.
-Qed.
-Hint Resolve Safe_cond_false_k.
-
-Ltac use_disjoint_trans'' := 
-  match goal with
-    | H : disjoint ?A ?B |- disjoint ?C _ =>
-      match A with context [ C ] =>
-        eapply (@disjoint_trans_lr _ A B C _ H)
-      end 
-    | H : disjoint ?A ?B |- disjoint (?C1 ++ ?C2) _ =>
-      match A with context [ C1 ] =>
-        match A with context [ C2 ] =>
-          eapply (@disjoint_trans_lr _ A B (C1 ++ C2) _ H)
-        end
-      end 
-  end.
-Hint Extern 1 => use_disjoint_trans''.
-
-Ltac change_rp :=
-  match goal with
-    H : ?SPECS (sel ?VS1 "rp") = Some _ |- ?SPECS (sel ?VS2 "rp") = Some _ =>
-      replace (sel VS2 "rp") with (sel VS1 "rp") by (symmetry; eapply changed_in_inv; [ eauto | ]; eapply in_tran_not; [ | eauto ]; eapply incl_tran; [ | eassumption ]; eauto)
-  end.
-Local Notation "'tmps' s" := (tempVars (depth s)) (at level 60).
-Local Notation "'etmps' s" := (tempVars (edepth s)) (at level 60).
-Ltac change_RunsTo_for_goal :=
-  match goal with
-    H : RunsTo _ ?S ?VS1 _ |- context [ RunsTo _ ?S ?VS1' _ ] => generalize H; eapply RunsTo_immune with (vs1' := VS1') in H; intros
-  end.
-
-Local Notation agree_in := unchanged_in.
-Local Notation agree_except := changed_in.
-Definition st_agree_except (v1 v2 : st) vars := agree_except (fst v1) (fst v2) vars /\ snd v1 = snd v2.
-Local Notation "b [ vars => c ]" := (merge c b vars) (no associativity, at level 60).
-Infix "==" := VariableLemmas.equiv.
-Local Notation "v1 =~= v2 [^ except ]" := (st_agree_except v1 v2 except) (no associativity, at level 60).
-
-Lemma st_agree_except_symm : forall v1 v2 ex, v1 =~= v2 [^ex] -> v2 =~= v1 [^ex].
-  unfold st_agree_except; intuition.
-Qed.
-Lemma RunsToRelax_immune : forall fs s v1 v2 v1' v2', 
-  fs ~:~ v1 ~~ s ~~> v2 ->
-  v1' =~= v1 [^ tmps s] -> 
-  v2' =~= v2 [^ tmps s] ->
-  disjoint (footprint s) (tmps s) ->
-  fs ~:~ v1' ~~ s ~~> v2'.
-  intros; eapply st_agree_except_symm in H0; eapply st_agree_except_symm in H1; unfold st_agree_except, RunsToRelax in *; openhyp; change_RunsTo_for_goal; eauto; openhyp; descend.
-  eauto.
-  use_changed_in_eval; eauto; eapply changedVariables_symm in H0; eauto.
-  congruence.
-Qed.
-Ltac change_RunsTo_to t :=
-  match goal with
-    H : RunsTo _ ?S ?VS1 _ |- _ => generalize H; eapply RunsTo_immune with (vs1' := t) in H; intros
-  end.
-Local Notation "fs -:- v1 -- s --> v2" := (RunsTo fs s v1 v2) (no associativity, at level 60).
-Lemma inversion_RunsTo_seq : forall fs a b v1 v2, fs -:- v1 -- a;: b --> v2 -> exists v, fs -:- v1 -- a --> v /\ fs -:- v -- b --> v2.
-  inversion 1; eauto.
-Qed.
-Hint Resolve Max.max_lub.
-Lemma st_agree_except_refl : forall v ex, v =~= v [^ex].
-  unfold st_agree_except; eauto.
-Qed.
-Hint Resolve st_agree_except_refl.
-Lemma RunsToRelax_cond_true' : forall fs e t f k v1 v2,
-  fs ~:~ v1 ~~ t;: k ~~> v2 ->
-  wneb (v1[(e)]) $0 = true ->
-  fs ~:~ v1 ~~ Conditional e t f;: k ~~> v2.
-  unfold RunsToRelax; intros; openhyp; auto_apply_in inversion_RunsTo_seq; openhyp; descend; simpl in *; eauto 6.
-Qed.
-Hint Resolve RunsToRelax_cond_true'.
-Lemma RunsToRelax_cond_true : forall fs e t f k v1 v1' v2,
-  let s := Conditional e t f;: k in
-    fs ~:~ v1 ~~ t;: k ~~> v2 ->
-    v1' =~= v1 [^etmps e] ->
-    wneb (v1'[(e)]) $0 = true ->
-    disjoint (footprint s) (tmps s) ->
-    fs ~:~ v1' ~~ s ~~> v2.
-  intros; eapply RunsToRelax_immune; unfold s, st_agree_except in *; openhyp; descend; simpl in *; eauto.
-Qed.
-Lemma RunsToRelax_cond_false' : forall fs e t f k v1 v2,
-  fs ~:~ v1 ~~ f;: k ~~> v2 ->
-  wneb (v1[(e)]) $0 = false ->
-  fs ~:~ v1 ~~ Conditional e t f;: k ~~> v2.
-  unfold RunsToRelax; intros; openhyp; auto_apply_in inversion_RunsTo_seq; openhyp; descend; simpl in *; eauto 6.
-Qed.
-Hint Resolve RunsToRelax_cond_false'.
-Lemma RunsToRelax_cond_false : forall fs e t f k v1 v1' v2,
-  let s := Conditional e t f;: k in
-    fs ~:~ v1 ~~ f;: k ~~> v2 ->
-    v1' =~= v1 [^etmps e] ->
-    wneb (v1'[(e)]) $0 = false ->
-    disjoint (footprint s) (tmps s) ->
-    fs ~:~ v1' ~~ s ~~> v2.
-  intros; eapply RunsToRelax_immune; unfold s, st_agree_except in *; openhyp; descend; simpl in *; eauto.
-Qed.
-Hint Unfold st_agree_except.
-Hint Resolve RunsToRelax_cond_true RunsToRelax_cond_false.
-
-Local Notation "v [ e ]" := (exprDenote e v) (no associativity, at level 60).
-Lemma Safe_assign : forall fs var e k vs arrs,
-  Safe fs (var <- e;: k) (vs, arrs)
-  -> Safe fs k (upd vs var (vs[e]), arrs).
-  inversion 1; eauto.
-Qed.
-Lemma in_not_in_ne : forall A ls (a b : A), In a ls -> ~ In b ls -> a <> b.
-  intuition.
-Qed.
-
-Local Notation "a [ i ] *<- e" := (Syntax.WriteAt a i e) (at level 60).
-
-Fixpoint denote_sem s (v : st) := 
-  match s with
-    | var <- e => (upd (fst v) var (fst v[e]), snd v)
-    | arr[idx] *<- val => 
-      let (vs, arrs) := v in 
-        let arr_v := exprDenote arr vs in
-          let idx_v := exprDenote idx vs in
-            let value_v := exprDenote val vs in
-              let new_arr := Array.upd (snd arrs arr_v) idx_v value_v in
-                (vs, (fst arrs, WDict.upd (snd arrs) arr_v new_arr))
-    | Syntax.ReadAt var arr idx =>
-      let (vs, arrs) := v in
-        let arr_v := exprDenote arr vs in
-          let idx_v := exprDenote idx vs in
-            let value_v := Array.sel (snd arrs arr_v) idx_v in  
-              (Locals.upd vs var value_v, arrs)
-    | Syntax.Len var arr => 
-      let (vs, arrs) := v in
-        let arr_v := exprDenote arr vs in
-          let len := natToW (length (snd arrs arr_v)) in
-            (Locals.upd vs var len, arrs)
-    | _ => v
-  end.
-
-Lemma RunsToRelax_assign : forall fs var e k v1 v2 v3,
-  fs ~:~ v2 ~~ k ~~> v3 ->
-  denote_sem (var <- e) v1 =~= v2 [^etmps e] ->
-  disjoint (footprint k) (etmps e) ->
-  fs ~:~ v1 ~~ var <- e;: k ~~> v3.
-  intros; eapply st_agree_except_symm in H0; unfold denote_sem, RunsToRelax, st_agree_except in *; openhyp; change_RunsTo_to (denote_sem (var <- e) v1); eauto; openhyp; destruct v1; simpl in *; descend.
-  eauto.
-  eapply changedVariables_symm in H0; use_changed_in_eval; eauto.
-  congruence.
-Qed.
-
-Lemma Safe_assoc_left : forall fs a b c v, Safe fs (a;: b;: c) v -> Safe fs (a;: (b;: c)) v.
-  clear; intros; inv_Safe; subst; inversion H; subst; econstructor; [ | intros; econstructor ]; eauto.
-Qed.
-Ltac true_not_false :=
-  match goal with
-    H1 : ?A = true, H2 : ?A = false |- _ => eapply Bool.eq_true_false_abs in H1; intuition
-  end.
-Hint Extern 1 => true_not_false.
-Lemma Safe_loop_true : forall fs e b v,
-  Safe fs (Loop e b) v ->
-  wneb (v[(e)]) $0 = true ->
-  Safe fs (b;: Loop e b) v.
-  intros.
-  inv_Safe.
-  unfold statement0 in *.
-  rewrite <- H2 in *.
-  eauto.
-  eauto.
-Qed.
-Hint Resolve Safe_loop_true.
-Lemma RunsTo_loop_true : forall fs e b v1 v2,
-  fs -:- v1 -- b;: Loop e b --> v2 ->
-  wneb (v1[(e)]) $0 = true ->
-  fs -:- v1 -- Loop e b --> v2.
-  clear; intros; eapply inversion_RunsTo_seq in H; openhyp; eauto.
-Qed.
-Hint Resolve RunsTo_loop_true.
-Lemma Safe_loop_true_k : forall fs e b k v, 
-  Safe fs (Loop e b;: k) v ->
-  wneb (v[(e)]) $0 = true ->
-  Safe fs (b;: (Loop e b;: k)) v.
-  intros.
-  inv_Safe.
-  subst.
-  inversion H3; try (unfold vals in *; congruence).
-  subst b.
-  subst v.
-  econstructor.
-  eauto.
-  intros.
-  econstructor; eauto.
-Qed.
-Hint Resolve Safe_loop_true_k.
-Local Notation agree_except_trans := changedVariables_trans.
-Definition tmps_diff big small := tempChunk (depth small) (depth big - depth small).
-Lemma agree_except_app_comm : forall vs1 vs2 a b,
-  agree_except vs1 vs2 (a ++ b) ->
-  agree_except vs1 vs2 (b ++ a).
-  intros; eauto.
-Qed.
-Lemma merge_comm : forall v vars1 v1 vars2 v2,
-  disjoint vars1 vars2 ->
-  v [vars1 => v1] [vars2 => v2] == v [vars2 => v2] [vars1 => v1].
-  intros.
-  unfold VariableLemmas.equiv, changedVariables.
-  intros.
-  contradict H0.
-  destruct (In_dec string_dec x vars1).
-  destruct (In_dec string_dec x vars2).
-  unfold disj in *.
-  contradict H.
-  eauto.
-  rewrite sel_merge by eauto.
-  rewrite sel_merge_outside by eauto.
-  rewrite sel_merge by eauto.
-  eauto.
-  destruct (In_dec string_dec x vars2).
-  rewrite sel_merge_outside by eauto.
-  rewrite sel_merge by eauto.
-  rewrite sel_merge by eauto.
-  eauto.
-  rewrite sel_merge_outside by eauto.
-  rewrite sel_merge_outside by eauto.
-  rewrite sel_merge_outside by eauto.
-  rewrite sel_merge_outside by eauto.
-  eauto.
-Qed.
-Lemma equiv_merge_equiv : forall v1 v2 vars v,
-  v1 == v2 ->
-  v1 [vars => v] == v2 [vars => v].
-  intros; eapply two_merge_equiv; eauto.
-Qed.
-Lemma RunsToRelax_seq_fwd : forall fs a b v1 v2,
-  fs ~:~ v1 ~~ a;: b ~~> v2 ->
-  disjoint (footprint (a;: b)) (tmps (a;: b)) ->
-  exists v, fs ~:~ v1 ~~ a ~~> v /\ fs ~:~ v ~~ b ~~> v2.
-  clear.
-  unfold RunsToRelax; intros.
-  openhyp.
-  eapply inversion_RunsTo_seq in H.
-  openhyp.
-  simpl in *.
-  destruct (le_lt_dec (depth a) (depth b)).
-  exists (fst x0 [tmps a => fst v2], snd x0).
-  split.
-  descend; eauto.
-  eapply changed_merge_fwd.
-  change_RunsTo_for_goal.
-  openhyp.
-  simpl in *.
-  descend; eauto.
-  use_changed_in_eval.
-  eapply changed_trans_l.
-  eapply changed_merge_bwd.
-  eauto.
-  eauto.
-  eauto.
-  congruence.
-  simpl.
-  eapply changed_unchanged.
-  eapply changed_merge_fwd.
-  eauto.
-  eauto.
-  set (diff := tmps_diff a b).
-  exists (fst x0 [diff => fst v2], snd x0).
-  split.
-  descend; eauto.
-  eapply agree_except_trans.
-  2 : eapply changed_merge_fwd.
-  eauto.
-  eauto.
-  unfold diff, tmps_diff.
-  eapply incl_tempChunk2.
-  omega.
-  change_RunsTo_for_goal.
-  openhyp.
-  simpl in *.
-  descend; eauto.
-  eapply changed_trans_l.
-  Focus 2.
-  eapply changed_merge.
-  eapply agree_except_app_comm.
-  rewrite Max.max_l in * by eauto.
-  erewrite <- split_tmps.
-  eauto.
-  eauto.
-  2 : eapply List.incl_refl.
-  eapply changedVariables_incl.
-  2 : eauto.
-  eapply VariableLemmas.equiv_trans.
-  eauto.
-  apply_in_all RunsTo_footprint.
-  eapply VariableLemmas.equiv_trans.
-  eapply VariableLemmas.equiv_symm.
-  eapply merge_comm.
-  unfold diff, tmps_diff.
-  eauto.
-  unfold diff, tmps_diff.
-  eapply equiv_merge_equiv.
-  eapply changed_merge.
-  eauto.
-  congruence.
-  simpl.
-  unfold diff, tmps_diff.
-  eapply changed_unchanged.
-  eapply changed_merge_fwd.
-  eauto.
-  eauto.
-Qed.
-Lemma RunsToRelax_seq_bwd : forall fs a b v1 v2 v3,
-  fs ~:~ v1 ~~ a ~~> v2 ->
-  fs ~:~ v2 ~~ b ~~> v3 ->
-  disjoint (footprint (a;: b)) (tmps (a;: b)) ->
-  fs ~:~ v1 ~~ a;: b ~~> v3.
-  unfold RunsToRelax; intros; openhyp; generalize dependent H; simpl in *; change_RunsTo_to x0; eauto; openhyp; descend; eauto; try use_changed_in_eval; eauto.
-  congruence.
-Qed.
-Hint Resolve RunsToRelax_seq_bwd.
-Lemma RunsToRelax_assoc_left : forall fs a b c v1 v2,
-  fs ~:~ v1 ~~ a;: (b;: c) ~~> v2 ->
-  disjoint (footprint (a;: (b;: c))) (tmps (a;: (b;: c))) ->
-  fs ~:~ v1 ~~ a;: b;: c ~~> v2.
-  clear; simpl; intros; eapply RunsToRelax_seq_fwd in H; eauto; openhyp; eapply RunsToRelax_seq_fwd in H1; eauto; openhyp; repeat eapply RunsToRelax_seq_bwd; repeat (simpl; eauto).
-Qed.
-Lemma RunsToRelax_loop_true : forall fs e b v1 v2, 
-  fs ~:~ v1 ~~ b;: Loop e b ~~> v2 -> 
-  wneb (v1[(e)]) $0 = true -> 
-  fs ~:~ v1 ~~ Loop e b ~~> v2.
-  unfold RunsToRelax; intros; openhyp; simpl in *; descend; eauto.
-Qed.
-Hint Resolve RunsToRelax_loop_true.
-Lemma RunsToRelax_loop_true_k : forall fs e b k v1 v2, 
-  let s := Loop e b;: k in
-    fs ~:~ v1 ~~ b;: s ~~> v2 -> 
-    wneb (v1[(e)]) $0 = true -> 
-    disjoint (footprint s) (tmps s) ->
-    fs ~:~ v1 ~~ s ~~> v2.
-  simpl; intros; eapply RunsToRelax_assoc_left in H; simpl; eauto; eapply RunsToRelax_seq_fwd in H; simpl; eauto; openhyp; eauto.
-Qed.
-Hint Resolve RunsToRelax_loop_true_k.
-
-Hint Resolve Safe_assoc_left.
-
-Local Notation skip := Syntax.Skip.
-
-Lemma RunsToRelax_skip : forall fs s v1 v2,
-  fs ~:~ v1 ~~ s ~~> v2 ->
-  fs ~:~ v1 ~~ skip;: s ~~> v2.
-  unfold RunsToRelax; intros; openhyp; descend; eauto.
-Qed.
-Hint Resolve RunsToRelax_skip.
-
-Lemma mult_S_distr : forall a b, a * S b = a + a * b.
-  intros; ring.
-Qed.
-
-Opaque star. (* necessary to use eapply_cancel *)
-
-Ltac eapply_cancel h specs st := let HP := fresh in let Hnew := fresh in
-  evar (HP : HProp); assert (interp specs (![HP] st)) as Hnew;
-    [ | eapply h in Hnew; [ | clear Hnew .. ] ]; unfold HP in *; clear HP; 
-      [ solve [try clear_imports; hiding ltac:(step auto_ext) ] | .. ].
-
-Ltac transit := 
-  match goal with
-    | H_interp : interp _ _, H : _ |- _ => eapply H in H_interp; clear H
-    | H_interp : interp ?SPECS (![_] ?ST), H : context [interp _ (![_] ?ST) -> _] |- _ => eapply_cancel H SPECS ST; clear H H_interp
-  end.
-
-Ltac try_post :=
-  try match goal with
-    H_interp : interp _ ?P |- _ =>
-      match P with
-        | context [ Exists ] => post
-      end
-  end.
-
-Lemma pack_pair' : forall A B (x : A * B), (let (x, _) := x in x, let (_, y) := x in y) = x.
-  destruct x; simpl; intuition.
-Qed.
-
-Lemma fold_second : forall A B (p : A * B), (let (_, y) := p in y) = snd p.
-  destruct p; simpl; intuition.
-Qed.
-
-Lemma fold_first : forall A B (p : A * B), (let (x, _) := p in x) = fst p.
-  destruct p; simpl; intuition.
-Qed.
-
-Ltac post_step := repeat first [ rewrite pack_pair' in * | rewrite fold_second in * | rewrite fold_first in *].
-
-Ltac not_mem_rv INST := 
-  match INST with
-    | context [LvMem ?LOC] =>
-      match LOC with
-        | context [Rv] => fail 2
-        | _ => idtac
-      end
-    | _ => idtac
-  end.
-
-Ltac pre_eval_auto := 
-  repeat 
-    match goal with
-      | H_eval : evalInstrs _ ?ST ?INST = _, H_interp : interp _ (![?P] (_, ?ST)) |- _ =>
-        match INST with
-          context [ Rv ] => 
-          match goal with
-            H_rv : Regs ST Rv = _ |- _ => not_mem_rv INST; post_step; generalize dependent H_rv
-          end
-        end
-      | H_eval : evalInstrs _ ?ST ?INST = _, H_interp : interp _ (![?P] (_, ?ST)) |- _ =>
-        match P with
-          context [ heap ?HEAP ] => 
-          match goal with
-            H_heap : HEAP = _ |- _ => post_step; generalize dependent H_heap
-          end
-        end
-    end.
-
-Ltac evaluate_hints hints :=
-  match goal with
-    H : evalInstrs _ ?ST _ = _ |- _ => generalize dependent H; evaluate hints; intro; evaluate auto_ext
-  end.
-
-Ltac my_evaluate hints :=
-  match goal with
-    | H: interp _ (![_](_, ?ST)), H_eval: evalInstrs _ ?ST ?INST = _ |- _  =>
-      match INST with
-        | context [LvMem (Reg Rv) ] => evaluate_hints hints
-        | _ => pre_eval_auto; evaluate hints
-      end
-  end.
-
-Ltac simpl_sp :=
-  repeat match goal with
-           H : (_, _) # Sp = _ |- _ => simpl in H
-         end.
-
-Ltac fold_length := 
-  change (fix length (l : list string) : nat :=
-    match l with
-      | nil => 0
-      | _ :: l' => S (length l')
-    end) with (@length string) in *.
-
-Lemma fold_4S : forall n, (S (S (S (S (4 * n))))) = (4 + (4 * n)).
-  eauto.
-Qed.
-
-Lemma Safe_ReadAt_safe_access : forall fs var arr idx v, 
-  Safe fs (Syntax.ReadAt var arr idx) v ->
-  safe_access (snd v) (exprDenote arr (fst v)) (exprDenote idx (fst v)).
-  intros; inv_Safe_clear; eauto.
-Qed.
-
-Lemma Safe_WriteAt_safe_access : forall fs arr idx val v, 
-  Safe fs (Syntax.WriteAt arr idx val) v ->
-  safe_access (snd v) (exprDenote arr (fst v)) (exprDenote idx (fst v)).
-  intros; inv_Safe_clear; eauto.
-Qed.
-
-Lemma Safe_ReadAt_k_safe_access : forall fs var arr idx v k, 
-  Safe fs (Syntax.ReadAt var arr idx;: k) v ->
-  safe_access (snd v) (exprDenote arr (fst v)) (exprDenote idx (fst v)).
-  intros; eapply Safe_seq_first in H; inv_Safe_clear; eauto.
-Qed.
-
-Lemma Safe_WriteAt_k_safe_access : forall fs arr idx val v k, 
-  Safe fs (Syntax.WriteAt arr idx val;: k) v ->
-  safe_access (snd v) (exprDenote arr (fst v)) (exprDenote idx (fst v)).
-  intros; eapply Safe_seq_first in H; inv_Safe_clear; eauto.
-Qed.
-
-Ltac not_exist t :=
-  match goal with
-    | H : t |- _ => fail 1
-    | |- _ => idtac
-  end.
-
-Ltac assert_new t := not_exist t; assert t.
-
-Ltac assert_new_as t name := not_exist t; assert t as name.
-
-Definition heap_tag arrs (_ _ : W) := heap arrs.
-
-Ltac set_all t := let name := fresh "t" in set (name := t) in *.
-
-Ltac clear_bad H_interp s :=
-  repeat 
-    match goal with
-      | H : context [changed_in _ _ _] |- _ => generalize H; clear H
-      | H : Regs ?ST Rv = _  |- _ => not_eq ST s; generalize H; clear H
-      | H : context [Safe _ _ _] |- _ => not_eq H H_interp; generalize H; clear H
-    end.
-
-Lemma Safe_Len_k_in : forall fs var ptr v k, 
-  Safe fs (Syntax.Len var ptr;: k) v ->
-  fst v[ptr] %in fst (snd v).
-  intros; eapply Safe_seq_first in H; inv_Safe_clear; eauto.
-Qed.
-
-Ltac simpl_interp :=
-  match goal with
-    | H: interp _ (![_](_, ?ST)), H_eval: evalInstrs _ ?ST _ = _ |- _  =>
-      simpl in H; try rewrite fold_4S in H
-  end.
-
-Ltac pre_eval :=
-  match goal with
-    | H: interp _ (![_](_, ?ST)), H_eval: evalInstrs _ ?ST _ = _ |- _  =>
-      try clear_imports; HypothesisParty H; prep_locals; clear_bad H ST;
-        simpl_interp; simpl_sp; try rewrite fold_4S in *
-  end.
-
-Ltac post_eval := intros; try fold (@length W) in *; post_step; try fold_length; try rewrite fold_4S in *.
-
-Definition heap_to_split arrs (_ : W) := heap arrs.
-  
-Ltac cond_gen := try
-  match goal with
-    | H_interp : interp _ (![_](_, ?ST)), H_eval : evalInstrs _ ?ST ?INST = _ |- _ =>
-      match INST with
-        | context [variablePosition ?vars ?s] => assert_new (In s vars)
-        | context [variableSlot ?s ?vars] => assert_new (In s vars)
-        | context [ LvMem (Reg Rv) ] =>
-          match goal with
-            | H : safe_access ?ARRS ?ARR ?IDX, H_rv : Regs ST Rv = _ |- _ =>
-              assert_new (Regs ST Rv = ARR ^+ $4 ^* IDX); [ | clear H_rv; replace (heap ARRS) with (heap_tag ARRS ARR IDX) in * by eauto; set_all ARR; set_all IDX ]
-            | H : ?ARR %in fst ?ARRS, H_rv : Regs ST Rv = _ |- _ =>
-              assert_new (Regs ST Rv = ARR ^- $4); [ | clear H_rv; replace (heap ARRS) with (heap_to_split ARRS ARR) in * by eauto; set_all ARR ]
-            | H : Safe _ (Syntax.ReadAt _ ?ARR ?IDX) ?ST |- _ => eapply Safe_ReadAt_safe_access in H; simpl in H
-            | H : Safe _ (Syntax.WriteAt ?ARR ?IDX _) ?ST |- _ => eapply Safe_WriteAt_safe_access in H; simpl in H
-            | H : Safe _ (Syntax.ReadAt _ ?ARR ?IDX;: _) ?ST |- _ => generalize H; eapply Safe_ReadAt_k_safe_access in H; simpl in H
-            | H : Safe _ (Syntax.WriteAt ?ARR ?IDX _;: _) ?ST |- _ => generalize H; eapply Safe_WriteAt_k_safe_access in H; simpl in H
-            | H : Safe _ (Syntax.Len _ ?ARR;: _) ?ST |- _ => generalize H; eapply Safe_Len_k_in in H; simpl in H
-          end
-      end; [ clear H_eval .. | cond_gen ]
-  end.
-
-Definition get_arr (arrs : arrays) addr := snd arrs addr.
-
-Definition add_arr arrs addr ls := (fst arrs %+ addr, WDict.upd (snd arrs) addr ls).
-
-Definition remove_arr (arrs : arrays) addr := (fst arrs %- addr, snd arrs).
-
-Lemma star_comm : forall a b, a * b ===> b * a.
-  clear; intros; sepLemma.
-Qed.
-
-Lemma star_cancel_left : forall a b c, b ===> c -> a * b ===> a * c.
-  clear; intros; sepLemma.
-Qed.
-
-Lemma star_cancel_right : forall a b c, b ===> c -> b * a ===> c * a.
-  clear; intros; sepLemma.
-Qed.
-
-(* starS_equiv has been added to Sets.v. This lemma can be deleted from here after updating bedrock repo *)
-Ltac to_himp := repeat intro.
-
-Ltac from_himp := match goal with
-                    | [ |- interp ?specs (?p ?x ?y ---> ?q ?x ?y) ] =>
-                      generalize dependent y; generalize dependent x; generalize dependent specs;
-                        change (p ===> q)
-                  end.
-
-Lemma starS_equiv : forall P a b, a %= b -> starS P a ===> starS P b.
-  clear.
-  intros.
-  unfold starS.
-  to_himp.
-  apply existsL.
-  intros.
-  apply existsR with x.
-  from_himp.
-  eapply star_cancel_right.
-  sepLemma.
-Qed.
-
-Lemma heap_equiv : forall a b, a %%= b -> heap a ===> heap b.
-  intros.
-  destruct a; destruct b.
-  unfold equiv in *.
-  simpl in H.
-  openhyp.
-  unfold heap.
-  eapply Himp_trans.
-  eapply starS_equiv.
-  eauto.
-  eapply starS_weaken.
-  intros.
-  unfold array_ptr.
-  rewrite H0.
-  eapply Himp_refl.
-  eauto.
-Qed.
-
-Lemma equiv_symm : forall a b, a %%= b -> b %%= a.
-  clear; unfold equiv, WMake.equiv; simpl; intros; firstorder.
-Qed.
-
-Hint Resolve equiv_symm.
-
-Definition trigger A (_ : A) := True.
-
-Lemma array_ptr_array_with_size : forall d ls p, array_ptr (WDict.upd d p ls) p = array_with_size ls p.
-  clear; intros; unfold array_ptr; rewrite WDict.sel_upd_eq; eauto.
-Qed.
-
-Lemma heap_bwd : forall arrs, trigger arrs -> (Ex arr_ptr, Ex old_arrs, Ex new_arr, [| arrs %%= add_arr old_arrs arr_ptr new_arr |] * [| ~ arr_ptr %in fst old_arrs |] * (heap old_arrs * array_with_size new_arr arr_ptr)) ===> heap arrs.
-  clear; intros.
-  cancel auto_ext.
-  post_step.
-  simpl in x.
-  destruct x0.
-  simpl in H1.
-  eapply Himp_trans.
-  Focus 2.
-  eapply heap_equiv.
-  eauto.
-  unfold add_arr; simpl.
-  eapply Himp_trans.
-  Focus 2.
-  eapply starS_add_bwd.
-  eauto.
-  rewrite array_ptr_array_with_size.
-  eapply Himp_trans.
-  eapply star_comm.
-  eapply star_cancel_right.
-  eapply starS_weaken.
-  intros.
-  unfold array_ptr.
-  rewrite WDict.sel_upd_ne.
-  eapply Himp_refl.
-  eauto.
-Qed.
-
-Ltac trigger_bwd Hprop :=
-  match Hprop with
-    context [ heap ?ARRS ] =>
-    assert (trigger ARRS) by (unfold trigger; trivial)
-  end.
-
-Lemma equiv_refl : forall a, a %%= a.
-  clear; unfold equiv; intros; firstorder.
-Qed.
-Hint Resolve equiv_refl.
-
-Hint Resolve in_not_in_ne.
-
-Local Notation delete := Syntax.Free.
-
-Lemma heap_fwd : forall arrs arr, arr %in fst arrs -> heap_to_split arrs arr ===> Ex new_arrs, [| new_arrs = remove_arr arrs arr |] * array_with_size (get_arr arrs arr) arr * heap new_arrs.
-  clear; intros.
-  cancel auto_ext.
-  unfold heap_to_split, heap, arrays in *.
-  destruct arrs.
-  simpl in *.
-  eapply Himp_trans.
-  eapply starS_del_fwd.
-  eauto.
-  replace (array_ptr d arr) with (array_with_size (d arr) arr) by eauto.
-  eapply star_comm.
-Qed.
-
-Lemma Safe_free_in : forall fs ptr v, Safe fs (delete ptr) v -> fst v [ptr] %in fst (snd v).
-  inversion 1; subst; eauto.
-Qed.
-Hint Resolve Safe_free_in.
-
-Lemma RunsTo_RunsToRelax : forall fs s v1 v2,
-  fs -:- v1 -- s --> v2 ->
-  fs ~:~ v1 ~~ s ~~> v2.
-  clear; unfold RunsToRelax; intro; descend; eauto.
-Qed.
-Hint Resolve RunsTo_RunsToRelax.
-
-Lemma heap_fwd_access : forall arrs arr idx, safe_access arrs arr idx -> heap_tag arrs arr idx ===> Ex new_arrs, [| new_arrs = remove_arr arrs arr |] * [| (idx < natToW (length (get_arr arrs arr)))%word |] * array_with_size (get_arr arrs arr) arr * heap new_arrs.
-  clear; intros.
-  cancel auto_ext.
-  unfold safe_access in *; simpl in *; openhyp; eauto.
-  unfold heap_tag, heap, arrays in *.
-  destruct arrs.
-  eapply Himp_trans.
-  eapply starS_del_fwd.
-  unfold safe_access in *; simpl in *; openhyp; eauto.
-  unfold get_arr; simpl.
-  replace (array_ptr d arr) with (array_with_size (d arr) arr) by eauto.
-  eapply star_comm.
-Qed.
-
-Lemma array_with_size_fwd : forall ls p, array_with_size ls p ===> let len := length ls in ([| p <> $8 /\ freeable (p ^- $8) (len + 2) /\ goodSize (len + 2) |] * (p ^- $8) =?> 1 * (p ^- $4) =*> natToW len * array ls p)%Sep.
-  clear; intros; unfold array_with_size; sepLemma.
-Qed.
-
-Lemma array_with_size_bwd : forall ls p, let len := length ls in ([| p <> $8 /\ freeable (p ^- $8) (len + 2) /\ goodSize (len + 2) |] * (p ^- $8) =?> 1 * (p ^- $4) =*> natToW len * array ls p)%Sep ===> array_with_size ls p.
-  clear; intros; unfold array_with_size; sepLemma.
-Qed.
-
-Definition hints_array_access_bwd : TacPackage.
-  prepare tt (heap_bwd, array_with_size_bwd).
-Defined.
-
-Ltac apply_save_in lemma hyp := generalize hyp; eapply lemma in hyp; intro.
-
-Ltac assert_sp P Q H_sp :=
-  match P with
-    context [ locals _ _ _ ?P_SP ] =>
-    match Q with
-      context [ locals _ _ _ ?Q_SP] =>
-      assert (Q_SP = P_SP) as H_sp
-    end
-  end.
-
-Ltac set_heap_goal :=
-  match goal with
-    |- context [ heap ?ARRS ] => set_all ARRS
-  end.
-
-Ltac set_heap_hyp :=
-  match goal with
-    H : context [ heap ?ARRS ] |- _ => set_all ARRS
-  end.
-
-Ltac set_array_hyp :=
-  match goal with
-    H : context [ array ?ARR ?PTR ] |- _ => set_all ARR; set_all PTR
-  end.
-
-Lemma not_in_remove_arr : forall arr arrs, ~ arr %in fst (remove_arr arrs arr).
-  intros; unfold remove_arr; simpl; eauto.
-Qed.
-
-Hint Resolve not_in_remove_arr.
-
-Lemma Safe_write_access : forall fs arr idx val vs arrs, 
-  Safe fs (Syntax.WriteAt arr idx val) (vs, arrs) ->
-  safe_access arrs (exprDenote arr vs) (exprDenote idx vs).
-  intros; inv_Safe_clear; eauto.
-Qed.
-Hint Resolve Safe_write_access.
-
-Lemma Safe_write_k : forall fs a i e k v, let s := a[i] *<- e in Safe fs (s;: k) v -> Safe fs k (denote_sem s v).
-  clear; simpl; destruct v; inversion 1; eauto.
-Qed.
-
-Definition hints_heap_bwd : TacPackage.
-  prepare tt heap_bwd.
-Defined.
-
-Definition hints_heap_fwd : TacPackage.
-  prepare heap_fwd tt.
-Defined.
-
-Definition hints : TacPackage.
-  prepare (heap_fwd, heap_fwd_access, array_with_size_fwd) tt.
-Defined.
-
-Hint Resolve in_tran_not.
-
-Lemma vars_require_imply : forall vars s1 s2, 
-  vars_require vars s1 -> 
-  List.incl (footprint s2) (footprint s1) ->
-  depth s2 <= depth s1 ->
-  vars_require vars s2.
-  clear; unfold vars_require; intros; openhyp; descend; eauto.
-Qed.
-
-Local Notation "'e_vars_require'" := CompileExpr.expr_vars_require.
-
-Lemma vars_require_imply_e : forall vars s e base, vars_require vars s -> List.incl (varsIn e) (footprint s) -> (base + edepth e <= depth s)%nat -> e_vars_require ("__reserved" :: "__arg" :: vars) e base.
-  clear; unfold vars_require, CompileExpr.expr_vars_require; simpl; intuition; eauto.
-Qed.
-
-Ltac unfold_copy_vars_require :=
-  match goal with
-    H : vars_require _ _ |- _ => generalize H; unfold vars_require in H; simpl in H; intro; openhyp
-  end.
-
-Ltac protect_hyps :=
-  repeat 
-    match goal with
-      | H : agree_except _ _ _ |- _ => generalize dependent H
-      | H : vars_require _ _ |- _ => generalize dependent H
-      | H : Regs _ Rv = _ |- _ => generalize dependent H
-      | H : safe_access _ _ _ |- _ => generalize dependent H
-      | H : _ %in _ |- _ => generalize dependent H
-      | H : Safe _ _ _ |- _ => generalize dependent H
-      | H : RunsToRelax _ _ _ _ |- _ => generalize dependent H
-    end.
-
-Ltac step_array_access := 
-  match goal with
-    H_interp : interp ?SPECS (![?P] ?ST) |- interp ?SPECS (![?Q] ?ST) => let H_sp := fresh in 
-      assert_sp P Q H_sp; [ .. | protect_hyps; generalize H_interp H_sp; clear; intros; trigger_bwd Q; set_array_hyp; set_heap_goal; step hints_array_access_bwd; post_step ]
-  end.
-
-Ltac changed_unchanged_disjoint :=
-  match goal with
-    H : disjoint ?A ?B |- agree_in _ _ _ => eapply changed_unchanged with (changed := B)
-  end.
-
-Ltac changed_in_inv_disjoint := 
-  match goal with
-    H : disjoint ?A ?B |- _ = _ => eapply changed_in_inv with (vars := B)
-  end.
-
-Ltac change_rp' :=
-  match goal with
-    H : ?SPECS (sel ?VS1 "rp") = Some _ |- ?SPECS (sel ?VS2 "rp") = Some _ =>
-      replace (sel VS2 "rp") with (sel VS1 "rp"); [ | symmetry; changed_in_inv_disjoint; [ | eapply in_tran_not; [ | eassumption ] ] ]
-  end.
-
-Ltac equiv_solver :=
-  match goal with
-    |- _ %%= add_arr ?ARRS _ _ => auto_unfold; no_question_mark; rewriter; unfold add_arr, remove_arr, equiv; simpl; to_tempOf; split; [ | intros; repeat f_equal; erewrite changed_in_inv by eauto; rewrite sel_upd_ne by eauto; erewrite changed_in_inv by eauto; rewrite sel_upd_eq by eauto]
-  end.
-
-Lemma Safe_read_access : forall fs var arr idx vs arrs, 
-  Safe fs (Syntax.ReadAt var arr idx) (vs, arrs) ->
-  safe_access arrs (exprDenote arr vs) (exprDenote idx vs).
-  intros; inv_Safe_clear; eauto.
-Qed.
-Hint Resolve Safe_read_access.
-
-Lemma Safe_read_k : forall fs var a i k v, let s := Syntax.ReadAt var a i in Safe fs (s;: k) v -> Safe fs k (denote_sem s v).
-  clear; simpl; destruct v; inversion 1; eauto.
-Qed.
-
-Ltac set_vs_hyp :=
-  match goal with
-    H : context [ locals _ ?VS _ _ ] |- _ => set_all VS
-  end.
-
-Ltac equiv_solver2 :=
-  match goal with
-    |- _ %%= add_arr ?ARRS _ _ => auto_unfold; no_question_mark; rewriter; unfold add_arr, remove_arr, equiv; simpl; to_tempOf; split; [ | intros; repeat f_equal]
-  end.
-
-Lemma upd_sel_equiv : forall d i i', WDict.upd d i (d i) i' = d i'.
-  clear; intros; destruct (weq i i').
-  rewrite WDict.sel_upd_eq; congruence.
-  rewrite WDict.sel_upd_ne; congruence.
-Qed.
-
-Ltac upd_chain_solver2 :=
-  match goal with
-    H1 : changed_in _ _ _, H2 : changed_in (upd _ _ _) _ _ |- changed_in _ _ _ => no_question_mark; simpl; iter_changed
-  end.
-
-Lemma Safe_len_in : forall fs var arr vs arrs, 
-  Safe fs (Syntax.Len var arr) (vs, arrs) ->
-  vs[arr] %in fst arrs.
-  intros; inv_Safe_clear; eauto.
-Qed.
-Hint Resolve Safe_len_in.
-
-Lemma Safe_len_k : forall fs var a k v, let s := Syntax.Len var a in Safe fs (s;: k) v -> Safe fs k (denote_sem s v).
-  clear; simpl; destruct v; inversion 1; eauto.
-Qed.
-
-Ltac vars_require_solver :=
-  match goal with
-    | H : vars_require _ _ |- vars_require _ _ => eapply vars_require_imply; repeat (simpl; eauto)
-    | H : vars_require _ _ |- e_vars_require _ _ _ => eapply vars_require_imply_e; repeat (simpl; eauto)
-  end.
-
-Ltac RunsToRelax_solver :=
-  match goal with
-    H : _ ~:~ _ ~~ ?S ~~> ?ST |- _ ~:~ _ ~~ ?S ~~> ?ST =>
-      eapply RunsToRelax_immune; [ eassumption | unfold st_agree_except; repeat split .. | ]
-  end.
-
-Ltac Safe_cond_solver :=
-  match goal with
-    H : Safe _ (Conditional _ _ _;: _) (?ST1, _) |- Safe _ _ _ =>
-      eapply Safe_immune with (vs1 := ST1); [ | use_changed_unchanged; simpl; eapply disjoint_trans_lr]
-  end.
-
-Ltac RunsToRelax_seq_solver :=
-  match goal with
-    H : _ ~:~ _ ~~ _;: (_;: _) ~~> _ |- _ ~:~ _ ~~ _;: _;: _ ~~> _ =>
-      eapply RunsToRelax_assoc_left; simpl
-  end.
-
-Ltac rv_solver' :=
-  match goal with
-    | H:Regs ?ST Rv = _ |- Regs ?ST Rv = _ => pattern_l; rewriter
-    | H:Regs ?ST Rv = _ |- _ = Regs ?ST Rv => pattern_r; rewriter
-    | H:_ = Regs ?ST Rv |- Regs ?ST Rv = _ => pattern_l; rewriter_r
-    | H:_ = Regs ?ST Rv |- _ = Regs ?ST Rv => pattern_r; rewriter_r
-  end.
-
-Ltac RunsToRelax_assign_solver :=
-  match goal with
-    H : _ ~:~ _ ~~ ?K ~~> _ |- _ ~:~ _ ~~ _ <- _;: ?K ~~> _ =>
-      eapply RunsToRelax_assign; [ eassumption | unfold st_agree_except | ]; simpl
-  end.
-
-Ltac Safe_assign_solver :=
-  match goal with
-    H : Safe _ (_ <- _;: ?K) _ |- Safe _ ?K _ =>
-      eapply Safe_immune; [ eapply Safe_assign; eassumption | eapply changed_unchanged; [ rewriter; use_changed_in_upd_same | ] ]
-  end.
-
-Ltac rp_upd_solver :=
-  match goal with
-    |- ?A = Some _ =>
-    match A with
-      context [ upd ] =>
-      match A with
-        context [ "rp" ] =>
-        rewrite sel_upd_ne; [ change_rp' | eapply in_not_in_ne ]
-      end
-    end
-  end.
-
-Local Notation agree_except_symm := changedVariables_symm.
-
-Ltac RunsToRelax_Stuff_solver :=
-  eapply RunsToRelax_seq_bwd; [ | eassumption | eauto ];
-    eapply RunsToRelax_immune; [ eapply RunsTo_RunsToRelax; econstructor; eauto | .. ];
-      [ | unfold st_agree_except; repeat split; simpl | ];
-      unfold st_agree_except; simpl; intuition eauto.
-
-Ltac do_RunsToRelax_Read_Write_solver := eapply RunsToRelax_seq_bwd; [ | eassumption | ..]; [ eapply RunsToRelax_immune; [ eapply RunsTo_RunsToRelax; econstructor; eauto | .. ]; [ | unfold st_agree_except; repeat split; simpl; eapply agree_except_symm | ] | ].
-
-Ltac RunsToRelax_Read_Write_solver :=
-  match goal with
-    | |- _ ~:~ _ ~~ _ [ _ ] *<- _;: _ ~~> _ => do_RunsToRelax_Read_Write_solver
-    | |- _ ~:~ _ ~~ Syntax.ReadAt _ _ _;: _ ~~> _ => do_RunsToRelax_Read_Write_solver
-    | |- _ ~:~ _ ~~ Syntax.Len _ _;: _ ~~> _ => do_RunsToRelax_Read_Write_solver
-  end.
-
-Ltac freeable_goodSize_solver :=
-  match goal with
-    | |- freeable _ _ => auto_unfold; rewrite upd_length in *
-    | |- goodSize _ => auto_unfold; rewrite upd_length in *
-  end.
-
-Ltac himp_length_solver :=
-  match goal with
-    |- (himp _ (_ =*> natToW (length ?A)) (_ =*> natToW (length ?B)))%Sep =>
-    unfold B; repeat hiding ltac:(step hints_array_access_bwd)
-  end.
-
-Ltac equiv_solver2' :=
-  match goal with
-    |- _ %%= add_arr _ _ _ =>
-    equiv_solver2; [ | unfold get_arr; symmetry; eapply upd_sel_equiv ]
-  end.
-
-Ltac pick_Safe := 
-  match goal with
-    | H : Safe _ (_ [ _ ] *<- _;: ?K) _ |- Safe _ ?K _ =>
-      eapply Safe_write_k in H; eapply Safe_immune; [ eassumption | ]
-    | H : Safe _ (Syntax.ReadAt _ _ _;: ?K) _ |- Safe _ ?K _ =>    
-      eapply Safe_read_k in H; eapply Safe_immune; [ eassumption | ]
-    | H : Safe _ (Syntax.Len _ _;: ?K) _ |- Safe _ ?K _ =>    
-      eapply Safe_len_k in H; eapply Safe_immune; [ eassumption | ]
-    | H : Safe _ (Syntax.Assignment _ _;: ?K) _ |- Safe _ ?K _ =>    
-      eapply Safe_assign in H; eapply Safe_immune; [ eassumption | ]
-  end.
-
-Ltac pre_eauto := try first [
-  use_disjoint_trans' |
-  use_Safe_immune2 |
-  extend_runs_loop_partially |
-  use_changed_in_eval |
-  arrays_eq_solver |
-  format_solver |
-  use_changed_in_upd_same |
-  not_in_solver |
-  equiv_solver |
-  upd_chain_solver |
-  arrays_eq_solver2 |
-  RunsTo_Malloc
-  ].
-
-Lemma mult_S_distr_inv : forall a b, a + a * b = a * S b.
-  intros; ring.
-Qed.
-
-Lemma wplus_wminus : forall (a b : W), a ^+ b ^- b = a.
-  intros; words.
-Qed.
-
-Ltac rewrite_expr :=
-  match goal with
-    | H : context [exprDenote ?E ?VS1] |- context [exprDenote ?E ?VS2] => not_eq VS1 VS2; rewrite (@unchanged_exprDenote _ VS1 VS2)
-  end.
-
-Ltac change_locals ns' avail' :=
-  match goal with
-    H : context[locals ?ns ?vs ?avail ?p] |- _ =>
-      let offset := eval simpl in (4 * List.length ns) in
-        change (locals ns vs avail p) with (locals_call ns vs avail p ns' avail' offset) in H; assert (ok_call ns ns' avail avail' offset)%nat
-  end.
-
-Ltac change_sp :=
-  match goal with
-    Hinterp : interp _ (![ ?P ] (_, ?ST)), Heval : evalInstrs _ ?ST _ = _ |- _ =>
-      match P with
-        context [ Regs ?ST2 Sp ] => not_eq ST ST2; replace (Regs ST2 Sp) with (Regs ST Sp) in Hinterp by words
-      end
-  end.
-
-Ltac generalize_sp :=
-  repeat match goal with
-           H : Regs _ Sp = Regs _ Sp |- _ => generalize dependent H
-         end.
-
-Ltac agree_in_solver :=
-  match goal with
-    |- agree_in _ _ _ => changed_unchanged_disjoint; [ iter_changed; incl_app_solver | .. ]
-  end.
-
-Ltac use_Safe_immune' :=
-  match goal with
-    H : Safe _ ?S (_, ?A) |- Safe _ ?S (_, ?A) =>
-      eapply Safe_immune; [ eassumption | .. ]; agree_in_solver
-  end.
-
-Ltac ok_call_solver :=
-  match goal with
-    |- ok_call _ _ _ _ _ =>
-    repeat split; simpl; unfold MIN_RESERVED in *; eauto; NoDup
-  end.
-
-Ltac myPost := autorewrite with sepFormula in *; unfold substH in *; simpl in *.
-
-Lemma aug_rp_not_in : forall vars, ~ In "rp" vars -> ~ In "rp" ("__reserved" :: "__arg" :: vars).
-  simpl; intuition.
-Qed.
-
-Ltac prep_rp :=
-  match goal with 
-    H : ~ In "rp" ?VARS |- _ =>
-      match VARS with
-        | context ["__reserved"] => fail 1
-        | _ => eapply aug_rp_not_in in H
-      end
-  end.
-
-Hint Resolve heap_star_not_in.
-
-Ltac rearrange_heap :=
-  match goal with
-    H : interp ?SPECS (![?P] ?ST) |- _ =>
-      match P with
-        context [ heap ?ARRS ] =>
-        match P with 
-          context [ array_with_size ?LS ?PTR ] =>
-          rearrange_stars (heap ARRS * array_with_size LS PTR)%Sep
-        end
-      end
-  end.
-
-Lemma not_in_reserved_arg : forall vars, ~ In "__reserved" vars -> ~ In "__reserved" ("__arg" :: vars).
-  simpl; intuition.
-Qed.
-
-Hint Resolve not_in_reserved_arg.
-
-Lemma Safe_Malloc_goodSize : forall fs var size v, Safe fs (Syntax.Malloc var size) v -> let size_v := exprDenote size (fst v) in goodSize (wordToNat size_v + 2).
-  inversion 1; subst; eauto.
-Qed.
-
-Hint Resolve Safe_Malloc_goodSize.
-
-Lemma Safe_malloc_goodSize : forall fs var size vs arrs, Safe fs (Syntax.Malloc var size) (vs, arrs) -> let size_v := exprDenote size vs in goodSize (wordToNat size_v + 2).
-  intros; eapply (@Safe_Malloc_goodSize _ _ _ (vs, arrs)); eauto.
-Qed.
-
-Hint Resolve Safe_malloc_goodSize.
-
-Ltac clear_or :=
-  repeat match goal with 
-           H : _ \/ _ |- _ => clear H 
-         end.
-
-Ltac simpl_vars :=
-  repeat match goal with 
-           | H : context [footprint _] |- _ => progress simpl in H
-           | H : context [tmps _] |- _ => progress simpl in H
-         end.
-
-Ltac tempOf_in_ext_solver :=
-  match goal with
-    |- In (tempOf _) ("__reserved" :: "__arg" :: ?VARS) =>
-    eapply In_incl with (ls1 := VARS)
-  end.
-
-Ltac replace_reserved :=
-  match goal with
-    H : context [sel ?VS1 "__reserved"] |- context [sel ?VS2 "__reserved"] =>
-      not_eq VS1 VS2; replace (sel VS2 "__reserved") with (sel VS1 "__reserved") in *
-  end.
-
-Lemma ignore_premise : forall pc state specs (P Q : PropX pc state),
-  interp specs Q
-  -> interp specs (P ---> Q).
-  intros; apply Imply_I; apply interp_weaken; assumption.
-Qed.
-
-Ltac step_himp_helper :=
-  match goal with
-    |- himp _ ?A ?B =>
-    match B with
-      context [locals ?VARS ?VS1 _ ?SP1] =>
-      match A with
-        context [locals VARS ?VS2 _ ?SP2] =>
-        match A with
-          context [locals ?VARS2 _ _ ?SP3] =>
-          not_eq VARS VARS2; replace SP1 with SP2; replace SP3 with (SP2 ^+ natToW (4 * length VARS)); replace VS1 with VS2
-        end
-      end
-    end
-  end.
-
-Ltac sel_eq_solver :=
-  match goal with
-    |- sel _ ?V = sel _ ?V => symmetry; changed_in_inv_disjoint
-  end.
-
-Ltac pre_eauto2 := try first [
-  ok_call_solver |
-  use_Safe_immune2 |
-  (format_solver; incl_app_solver) |
-  equiv_solver |
-  vars_require_solver |
-  RunsToRelax_solver | 
-  rp_upd_solver |
-  change_rp' |
-  rv_solver' |
-  Safe_cond_solver |
-  RunsToRelax_seq_solver |
-  RunsToRelax_assign_solver |
-  Safe_assign_solver | 
-  RunsToRelax_Read_Write_solver |
-  freeable_goodSize_solver |
-  changed_unchanged_disjoint |
-  himp_length_solver |
-  equiv_solver2' |
-  use_Safe_immune' |
-  sel_eq_solver |
-  tempOf_in_ext_solver
-  ].
-
-Lemma four_out : forall n, 4 * (S (S (S n))) = 4 * 3 + 4 * n.
-  intros; omega.
-Qed.
-
-Ltac eval_instrs hints :=
-  match goal with
-    | H: interp _ (![_](_, ?ST)), H_eval: evalInstrs _ ?ST _ = _ |- _  =>
-      cond_gen; [ .. | let P := fresh "P" in
-        try match goal with
-              | [ _ : context[Safe ?fs _ _] |- _ ] => set (P := Safe fs) in *
-            end;
-        pre_eval;
-        try match goal with
-              | [ H : _ = Regs ?X Rv, H' : _ = Regs ?X Rv |- _ ] => generalize dependent H'
-            end;
-        my_evaluate hints;
-        try subst P;
-          post_eval; clear H_eval]
-  end.
-
-Ltac clear_specs :=
-  repeat
-    match goal with
-      | H : interp ?SPECS_H _ |- context [simplify ?SPECS _ _] => not_eq SPECS_H SPECS; clear H
-      | H : interp ?SPECS_H _ |- context [interp ?SPECS _] => not_eq SPECS_H SPECS; clear H
-    end.
-
-Ltac pre_eval_statement := intros; open_hyp; try_post.
-
-Ltac eval_statement := pre_eval_statement; transit; open_hyp; try_post.
-
-Ltac eval_step hints := first[eval_statement | try clear_imports; eval_instrs hints].
-
-
-
-Module CompileMalloc.
-Section CompileMalloc.
-
-  Variable vars : list string.
-  Variable var : string.
-  Variable size : Expr.
-  Variable k : Statement.
-
-  Definition postcond := inv vars k.
-
-  Definition s_k := var <- new size;: k.
-
-  Definition precond := inv vars s_k.
-
-  (* cope with an [evaluate] failure *)
-  Definition length_require A ls vs := @length A ls = wordToNat (vs[size]).
-
-  Definition vars := "__reserved" :: "__arg" :: vars.
-
-  Definition afterCall : assert :=
-    st ~> Ex fs, funcsOk (fst st) fs /\ ExX, Ex v : Semantics.st, Ex ls, Ex res,
-    let old_sp := st#Sp ^- natToW (4 * 3 + 4 * length vars) in
-    let addr := st#Rv in
-    ![^[locals ("rp" :: vars) (fst v) res old_sp * heap (snd v) * mallocHeap 0 * array_with_size ls addr * [| length_require ls (fst v) /\ res = wordToNat (sel (fst v) "__reserved") /\ MIN_RESERVED <= res /\ Safe fs s_k v |] ] * #0] st
-    /\ (sel (fst v) "rp", fst st) @@@ (st' ~> Ex v',
-      [| st'#Sp = old_sp |]
-      /\ ![^[locals ("rp" :: vars) (fst v') res st'#Sp * heap (snd v') * mallocHeap 0] * #1] st'
-      /\ [| RunsToRelax fs s_k v v' |]).
-
-  Variable imports : LabelMap.t assert.
-  Variable imports_global : importsGlobal imports.
-  Variable modName : string.
-
-  Definition verifCond pre :=
-    (LabelMap.find (elt:=assert) ("my_malloc"!"malloc")%SP imports = Some (Precondition my_mallocS None))
-    :: imply pre precond :: vars_require vars s_k :: nil.
-
-  Definition Seq2 := @Seq_ _ imports_global modName.
-
-  Definition Strline := Straightline_ imports modName.
-
-  Definition Skip := Straightline_ imports modName nil.
-
-  Fixpoint Seq ls :=
-    match ls with
-      | nil => Skip
-      | a :: ls' => Seq2 a (Seq ls')
-    end.
-
-  Definition SaveRv var := Strline (Assign (variableSlot var vars) (RvLval (LvReg Rv)) :: nil).
-
-  Definition exprCmd := CompileExpr.exprCmd imports_global modName vars.
-
-  Definition body := Seq (
-    exprCmd size 0
-    :: SaveRv (tempOf 0)
-      :: Strline (
-        IL.Binop Rv Sp Plus (natToW (4 * 3 + 4 * List.length vars))
-        :: Assign (LvMem (Indir Rv (natToW 4))) (RvLval (variableSlot (tempOf 0) vars))
-        :: IL.Binop Sp Sp Plus (natToW (4 * 3 + 4 * List.length vars))
-        :: nil)
-      :: Structured.Call_ imports_global modName ("my_malloc"!"malloc")%SP afterCall
-      :: Strline (
-        IL.Binop Sp Sp Minus (natToW (4 * 3 + 4 * List.length vars))
-        :: nil)
-      :: SaveRv var
-        :: nil).
-
-  Opaque mult.
-
-  Opaque variablePosition.
-
-  Opaque heap.
-
-  Ltac unfold_eval := unfold precond, postcond, inv, expr_runs_to, runs_to_generic, vars, MIN_RESERVED in *.
-
-  Lemma post_ok : forall (pre : assert) (specs : codeSpec W (settings * state))
-    (x : settings * state),
-    vcs (verifCond pre) ->
-    interp specs (Postcondition (body pre) x) -> interp specs (postcond x).
-
-    unfold verifCond, imply.
-    wrap0.
-
-    unfold_eval; unfold_copy_vars_require; clear_imports; myPost; prep_rp; repeat eval_step auto_ext.
-    eauto.
-
-    destruct x5.
-    simpl in *.
-    descend.
-    propxFo.
-    propxFo.
-    instantiate (2 := (_, add_arr a (Regs x2 Rv) x6)).
-    simpl in *.
-    match goal with
-      |- interp _ ?Q => trigger_bwd Q
-    end.
-    hiding ltac:(step hints_heap_bwd).
-    post_step.
-    rearrange_heap; auto_apply_in heap_star_not_in; eauto.
-    rewriter.
-    simpl.
-    rewrite sel_upd_ne.
-    eauto.
-    eauto.
-    eauto.
-    rewriter.
-    inv_Safe.
-    subst.
-    auto_apply.
-    econstructor.
-    rearrange_heap; auto_apply_in heap_star_not_in; eauto.
-    auto_apply_in Safe_seq_first.
-    eauto.
-    eauto.
-    simpl; rewrite sel_upd_ne; eauto.
-    step auto_ext.
-    clear_or.
-    step auto_ext.
-    step auto_ext.
-    repeat match goal with
-             | [ H : _ = _ |- _ ] => rewrite H
-           end.
-    assumption.
-    hiding ltac:(step auto_ext).
-    unfold s_k in *.
-    eapply RunsToRelax_seq_bwd.
-    2 : eauto.
-    rewriter.
-    eapply RunsTo_RunsToRelax.
-    unfold add_arr.
-    econstructor.
-    rearrange_heap; auto_apply_in heap_star_not_in; eauto.
-    auto_apply_in Safe_seq_first.
-    eauto.
-    eauto.
-    simpl.
-    eauto.
-
-  Qed.
-
-  Ltac eval_step2 hints := unfold locals_call in *; 
-    match goal with
-      | Hinterp : interp _ (![ ?P ] (_, ?ST)), Heval : evalInstrs _ ?ST ?INSTRS = _ |- _ =>
-        match INSTRS with
-          | context [ IL.Binop _ (RvLval (LvReg Sp)) Plus _ ] =>
-            change_locals ("rp" :: "n" :: nil) 8; [ clear Heval |repeat rewrite <- mult_plus_distr_l in *; simpl in *; change_sp; generalize_sp; eval_step hints ]
-        end
-      | _ => eval_step hints
-    end.
-
-  Lemma verifCond_ok : forall pre : assert, vcs (verifCond pre) -> vcs (VerifCond (body pre)).
-
-    unfold verifCond, imply.
-    wrap0; try match goal with
-                 | [ H : _ = Some _ |- _ ] => rewrite H
-               end; clear_imports.
-    Focus 4.
-    intros; post; unfold_eval; unfold_copy_vars_require; prep_rp;
-      repeat eval_step2 auto_ext; to_tempOf; pre_eauto2; eauto.
-
-    eexists.
-    eexists.
-    split.
-    clear_or.
-    post.
-    hiding ltac:(step auto_ext).
-    unfold s_k in *.
-    rewriter.
-    auto_apply_in Safe_seq_first.
-    eauto.
-    destruct x4.
-    simpl in *.
-    descend.
-    eauto.
-    unfold afterCall.
-    step auto_ext.
-    step auto_ext.
-
-    apply ignore_premise.
-    propxFo.
-
-    instantiate (6 := (_, _)).
-    simpl.
-    instantiate (3 := upd x7 "." (v[size])).
-    hiding ltac:(step auto_ext).
-    Focus 4.
-    unfold vars in *.
-    step_himp_helper.
-    unfold MIN_RESERVED in *.
-    replace_reserved.
-    hiding ltac:(step auto_ext).
-
-    to_tempOf; pre_eauto2; eauto.
-
-    f_equal; eauto.
-    rewriter; rewrite <- mult_plus_distr_l; rewrite wplus_wminus; eauto.
-    f_equal; eauto.
-
-    unfold length_require.
-    to_tempOf.
-    rewriter; symmetry; f_equal; eapply exprDenote_disjoint.
-    eauto.
-    eapply disjoint_trans_lr.
-    eauto.
-    eauto.
-    incl_app_solver; eauto.
-
-    replace_reserved.
-    eauto.
-    to_tempOf; pre_eauto2; eauto.
-
-    eapply Safe_immune.
-    eauto.
-    simpl in *.
-    to_tempOf.
-    eapply changed_unchanged.
-    eauto.
-    eapply disjoint_trans_lr.
-    eauto.
-    eauto.
-    incl_app_solver; eauto.
-
-    simpl.
-    rewrite sel_upd_ne by intuition.
-    change_rp.
-    eauto.
-
-    do 4 step auto_ext; [ repeat match goal with
-                                                 | [ H : _ = _ |- _ ] => rewrite H
-                                               end; rewrite four_out; words
-      | instantiate (1 := (_, _)); simpl; replace (sel x7 "__reserved") with (sel v "__reserved") in *; [hiding ltac:(step auto_ext) | .. ] | .. ]; destruct x12; pre_eauto2; simpl; to_tempOf; eauto; iter_changed; incl_app_solver; eauto.
-
-    unfold_eval; eval_step auto_ext; descend; repeat hiding ltac:(step auto_ext); pre_eauto2.
-    unfold_eval; unfold_copy_vars_require; prep_rp; repeat eval_step2 auto_ext; to_tempOf; pre_eauto2; info_eauto.
-    unfold_eval; unfold_copy_vars_require; prep_rp; repeat eval_step2 auto_ext; to_tempOf; pre_eauto2; info_eauto.
-    post; unfold_eval; unfold_copy_vars_require; prep_rp; repeat eval_step2 auto_ext; to_tempOf; pre_eauto2; info_eauto.
-    post; unfold_eval; unfold_copy_vars_require; prep_rp; repeat eval_step2 auto_ext; to_tempOf; pre_eauto2; info_eauto.
-    post; unfold_eval; unfold_copy_vars_require; prep_rp; repeat eval_step2 auto_ext; to_tempOf; pre_eauto2; info_eauto.
-  Qed.
-
-  Definition compile := Wrap imports imports_global modName body (fun _ => postcond) verifCond post_ok verifCond_ok.
-
-End CompileMalloc.
-End CompileMalloc.
-
-Module CompileFree.
-Section CompileFree.
-
-  Variable vars : list string.
-  Variable ptr : Expr.
-  Variable k : Statement.
-
-  Definition postcond := inv vars k.
-
-  Definition s_k := delete ptr;: k.
-
-  Definition precond := inv vars s_k.
-
-  Definition vars := "__reserved" :: "__arg" :: vars.
-
-  Definition afterCall : assert :=
-    st ~> Ex fs, funcsOk (fst st) fs /\ ExX, Ex v : Semantics.st, Ex res,
-    let old_sp := st#Sp ^- natToW (4 * (1 + length vars)) in
-    let ptr_v := v[(ptr)] in
-    ![^[locals ("rp" :: vars) (fst v) res old_sp * heap (remove_arr (snd v) ptr_v) * mallocHeap 0 * [| res = wordToNat (sel (fst v) "__reserved") /\ MIN_RESERVED <= res /\ Safe fs s_k v |] ] * #0] st
-    /\ (sel (fst v) "rp", fst st) @@@ (st' ~> Ex v',
-      [| st'#Sp = old_sp |]
-      /\ ![^[locals ("rp" :: vars) (fst v') res st'#Sp * heap (snd v') * mallocHeap 0] * #1] st'
-      /\ [| RunsToRelax fs s_k v v' |]).
-
-  Variable imports : LabelMap.t assert.
-  Variable imports_global : importsGlobal imports.
-  Variable modName : string.
-
-  Definition verifCond pre :=
-    (LabelMap.find (elt:=assert) ("my_free"!"free")%SP imports = Some (Precondition my_freeS None))
-    :: imply pre precond :: vars_require vars s_k :: nil.
-
-  Definition Seq2 := @Seq_ _ imports_global modName.
-
-  Definition Strline := Straightline_ imports modName.
-
-  Definition Skip := Straightline_ imports modName nil.
-
-  Fixpoint Seq ls :=
-    match ls with
-      | nil => Skip
-      | a :: ls' => Seq2 a (Seq ls')
-    end.
-
-  Definition SaveRv var := Strline (Assign (variableSlot var vars) (RvLval (LvReg Rv)) :: nil).
-
-  Definition exprCmd := CompileExpr.exprCmd imports_global modName vars.
-
-  Definition body := Seq (
-    exprCmd ptr 0
-    :: SaveRv (tempOf 0)
-    :: Strline (
-      IL.Binop Rv Sp Plus (natToW (4 * (1 + List.length vars)))
-      :: Assign (LvMem (Indir Rv (natToW 4))) (RvLval (variableSlot (tempOf 0) vars))
-      :: IL.Binop Sp Sp Plus (natToW (4 * (1 + List.length vars)))
-      :: nil)
-    :: Structured.Call_ imports_global modName ("my_free"!"free")%SP afterCall
-    :: Strline (
-      IL.Binop Sp Sp Minus (natToW (4 * (1 + List.length vars)))
-      :: nil)
-    :: nil).
-
-  Opaque mult.
-
-  Opaque variablePosition.
-
-  Opaque heap.
-
-  Lemma Safe_s_k_first : forall fs v a, Safe fs s_k (v, a)
-    -> v[ptr] %in fst a.
-    intros.
-    apply Safe_seq_first in H.
-    inversion H; auto.
-  Qed.
-
-  Hint Immediate Safe_s_k_first.
-
-  Lemma Safe_s_k_second : forall fs v a, Safe fs s_k (v, a)
-    -> Safe fs k (v, (fst a %- (v [ptr]), snd a)).
-    intros.
-    eapply Safe_seq_second; eauto.
-  Qed.
-
-  Hint Immediate Safe_s_k_second.
-
-  Ltac unfold_eval := unfold precond, postcond, inv, expr_runs_to, runs_to_generic, vars, MIN_RESERVED in *.
-
-  Lemma post_ok : forall (pre : assert) (specs : codeSpec W (settings * state))
-    (x : settings * state),
-    vcs (verifCond pre) ->
-    interp specs (Postcondition (body pre) x) -> interp specs (postcond x).
-
-    unfold verifCond, imply.
-    wrap0.
-    unfold_eval; unfold_copy_vars_require; clear_imports; myPost; prep_rp; repeat eval_step auto_ext.
-
-    destruct x4; simpl in *.
-    descend.
-    eauto.
-    hiding ltac:(step auto_ext).
-    instantiate (2 := (_, _)).
-    simpl.
-    hiding ltac:(step auto_ext).
-    eauto.
-    eauto.
-    unfold remove_arr; eauto.
-    eauto.
-    step auto_ext.
-    step auto_ext.
-    step auto_ext.
-    repeat match goal with
-             | [ H : _ = _ |- _ ] => rewrite H
-           end; assumption.
-    hiding ltac:(step auto_ext).
-    unfold s_k in *.
-    unfold remove_arr in *.
-    eapply RunsToRelax_seq_bwd; eauto.
-  Qed.
-
-  Ltac eval_step2 hints := unfold locals_call in *; 
-    match goal with
-      | Hinterp : interp _ (![ ?P ] (_, ?ST)), Heval : evalInstrs _ ?ST ?INSTRS = _ |- _ =>
-        match INSTRS with
-          | context [ IL.Binop _ (RvLval (LvReg Sp)) Plus _ ] =>
-            change_locals ("rp" :: "ptr" :: nil) 8; [ clear Heval |repeat rewrite <- mult_plus_distr_l in *; simpl in *; change_sp; generalize_sp; eval_step hints ]
-        end
-      | _ => eval_step hints
-    end.
-
-  Lemma verifCond_ok : forall pre : assert, vcs (verifCond pre) -> vcs (VerifCond (body pre)).
-
-    unfold verifCond, imply.
-    wrap0; try match goal with
-                 | [ H : _ = Some _ |- _ ] => rewrite H
-               end; clear_imports.
-    Focus 4.
-    intros; post; unfold_eval; unfold_copy_vars_require; prep_rp; repeat eval_step2 auto_ext; to_tempOf; pre_eauto2; info_eauto.
-
-    destruct x4; simpl in *.
-    descend.
-    replace (heap a) with (heap_to_split a (v[ptr])) in * by eauto.
-    assert (v[ptr] %in fst a) by eauto.
-    hiding ltac:(step hints_heap_fwd).
-    hiding ltac:(step hints_heap_fwd).
-    eauto.
-    unfold afterCall.
-    step auto_ext.
-    step auto_ext.
-    
-    apply ignore_premise; propxFo.
-
-    unfold_eval.
-    hiding ltac:(step auto_ext).
-    Focus 3.
-    unfold remove_arr.
-    rewrite_expr.
-    instantiate (1 := (_, _)).
-    simpl.
-    Ltac rewrite_upd_rv :=
-      match goal with
-        H : Regs ?ST Rv = _ |- context [ upd _ _ (Regs ?ST Rv) ] => rewrite H
-      end.
-
-    Ltac step_himp_helper :=
-      match goal with
-        |- himp _ ?A ?B =>
-        match B with
-          context [locals ?VARS ?VS1 _ ?SP1] =>
-          match A with
-            context [locals VARS ?VS2 _ ?SP2] =>
-            match A with
-              context [locals ?VARS2 _ _ ?SP3] =>
-              not_eq VARS VARS2; rewrite_upd_rv; replace SP1 with SP2; replace SP3 with (SP2 ^+ natToW (4 * length VARS))
-            end
-          end
-        end
-      end.
-
-    step_himp_helper.
-    hiding ltac:(step auto_ext).
-    instantiate (1 := upd x7 "." (v [ptr])).
-    replace_reserved.
-    hiding ltac:(step auto_ext).
-
-    to_tempOf; pre_eauto2; info_eauto.
-    iter_changed; eauto.
-    words.
-    to_tempOf; agree_in_solver; info_eauto.
-    simpl.
-    rewrite sel_upd_ne.
-    replace_reserved.
-    eauto.
-    to_tempOf; pre_eauto2; info_eauto.
-    intuition.
-    to_tempOf; pre_eauto2; info_eauto.
-    simpl; to_tempOf; pre_eauto2; info_eauto.
-
-    destruct x11; do 3 step auto_ext; [ repeat match goal with
-                                                 | [ H : _ = _ |- _ ] => rewrite H
-                                               end; rewrite four_out; words |
-    instantiate (1 := (_, _)); simpl; replace_reserved; [hiding ltac:(step auto_ext) | .. ] | .. ];
-      pre_eauto2; simpl; to_tempOf; eauto; iter_changed; incl_app_solver; eauto.
-
-    unfold_eval; eval_step auto_ext; descend; repeat hiding ltac:(step auto_ext); pre_eauto2.
-    unfold_eval; unfold_copy_vars_require; prep_rp; repeat eval_step2 auto_ext; to_tempOf; pre_eauto2; info_eauto.
-    unfold_eval; unfold_copy_vars_require; prep_rp; repeat eval_step2 auto_ext; to_tempOf; pre_eauto2; info_eauto.
-    post; unfold_eval; unfold_copy_vars_require; prep_rp; repeat eval_step2 auto_ext; to_tempOf; pre_eauto2; info_eauto.
-    post; unfold_eval; unfold_copy_vars_require; prep_rp; repeat eval_step2 auto_ext; to_tempOf; pre_eauto2; info_eauto.
-  Qed.
-
-  Definition compile := Wrap imports imports_global modName body (fun _ => postcond) verifCond post_ok verifCond_ok.
-
-End CompileFree.
-End CompileFree.
 
